examples/spinlock/spinlock2Script.sml
@@ -1,0 +1,1243 @@
+
+open HolKernel Parse boolLib bossLib;
+
+open rich_listTheory listTheory arithmeticTheory finite_mapTheory ;
+open bir_lifter_interfaceLib bir_promisingTheory ;
+open tracesTheory tracestepTheory spinlockTheory;
+
+(*
+ * spinlock correctness proof
+ *)
+
+val _ = new_theory "spinlock2";
+
+(*
+val _ = Parse.current_backend := PPBackEnd.vt100_terminal;
+val _ = set_trace "bir_inst_lifting.DEBUG_LEVEL" 2;
+
+val (bir_spinlockfull_progbin_def, bir_spinlockfull_prog_def, bir_is_lifted_prog_spinlockfull) = lift_da_and_store_mc_riscv
+          "spinlockfull"
+          "spinlockfull.da"
+          ((Arbnum.fromInt 0), (Arbnum.fromInt 0x1000000));
+*)
+
+(* simplifying terms through rewrites *)
+
+Triviality CONJ_EQ_NEQ_ELIM:
+  (!x v' v. x = v /\ x <> v' <=> x = v /\ v <> v')
+  /\ (!x v' v. x <> v' /\ x = v  <=> x = v /\ v <> v')
+  /\ (!x v' v A. x = v /\ x <> v' /\ A <=> x = v /\ v <> v' /\ A)
+  /\ (!x v' v A. x <> v' /\ x = v /\ A <=> v <> v' /\ x = v /\ A)
+  /\ (!x v' v B. B /\ x = v /\ x <> v' <=> B /\ x = v /\ v <> v')
+  /\ (!x v' v B. B /\ x <> v' /\ x = v <=> B /\ v <> v' /\ x = v )
+  /\ (!x v' v B. x = v /\ B /\ x <> v' <=> x = v /\ B /\ v <> v')
+  /\ (!x v' v B. x <> v' /\ B /\ x = v <=> v <> v' /\ B /\ x = v)
+  /\ (!x v' v A B. x = v /\ B /\ x <> v' /\ A <=> x = v /\ B /\ v <> v' /\ A)
+  /\ (!x v' v A B. x <> v' /\ B /\ x = v /\ A <=> v <> v' /\ B /\ x = v /\ A)
+  /\ (!x v' v A B. B /\ x = v /\ x <> v' /\ A <=> B /\ x = v /\ v <> v' /\ A)
+  /\ (!x v' v A B. B /\ x <> v' /\ x = v /\ A <=> B /\ v <> v' /\ x = v /\ A)
+Proof
+  fs[EQ_IMP_THM]
+QED
+
+Theorem ELIM_thms:
+  !P.
+  (!x v. x = v /\ P x <=> P v /\ x = v)
+  /\ (!x v. P x /\ x = v  <=> P v /\ x = v)
+
+  /\ (!x v A. x = v /\ A /\ P x <=> P v /\ x = v /\ A)
+  /\ (!x v A. x = v /\ P x /\ A <=> P v /\ x = v /\ A)
+  /\ (!x v A. P x /\ x = v /\ A <=> P v /\ x = v /\ A)
+  /\ (!x v A. P x /\ A /\ x = v <=> P v /\ x = v /\ A)
+
+  /\ (!x v A B. B /\ x = v /\ A /\ P x <=> P v /\ x = v /\ B /\ A)
+  /\ (!x v A B. B /\ x = v /\ P x /\ A <=> P v /\ x = v /\ B /\ A)
+  /\ (!x v A B. B /\ P x /\ x = v /\ A <=> P v /\ x = v /\ B /\ A)
+  /\ (!x v A B. B /\ P x /\ A /\ x = v <=> P v /\ x = v /\ B /\ A)
+
+  /\ (!x v A B C. B /\ x = v /\ C /\ P x /\ A <=> P v /\ x = v /\ B /\ C /\ A)
+Proof
+  fs[EQ_IMP_THM]
+QED
+
+(* generates various conjunction theorems with given term *)
+(*
+ val term = ``λx. v = x``
+ val term = ``λx. get_read_args v = x``
+  fun_eq_conjs term
+ *)
+fun fun_eq_conjs term =
+  let
+    val ty = type_of term
+    val thm =
+      ISPEC term ELIM_thms
+      (* int_arithTheory.CONJ_EQ_ELIM *)
+      |> SIMP_RULE (std_ss) []
+  in
+    map GEN_ALL $ CONJUNCTS thm
+  end
+
+(* conversion to removing evident inequalities, like  a <> 2
+ * in  |- P a <=> a = 1 /\ a <> 2  *)
+val CONJ_EQ_NEQ_conv = REPEATC $
+  ONCE_DEPTH_CONV (REWRITE_CONV $ CONJUNCTS CONJ_EQ_NEQ_ELIM)
+  THENC (SIMP_CONV (srw_ss()) [])
+  THENC
+  ONCE_DEPTH_CONV (REWRITE_CONV $ fun_eq_conjs ``λx. x:num <> v'``)
+  THENC (SIMP_CONV (srw_ss()) [])
+  THENC ONCE_DEPTH_CONV (REWRITE_CONV $ fun_eq_conjs ``λx. x:bir_label_t <> v'``)
+  THENC (SIMP_CONV (srw_ss()) [])
+  THENC ONCE_DEPTH_CONV (REWRITE_CONV $ fun_eq_conjs ``λi. EL i ls = x``)
+  THENC (SIMP_CONV (srw_ss()) [])
+  THENC ONCE_DEPTH_CONV (REWRITE_CONV $ fun_eq_conjs ``λe. get_fulfil_args e = x``)
+  THENC (SIMP_CONV (srw_ss()) [])
+  THENC ONCE_DEPTH_CONV (REWRITE_CONV $ fun_eq_conjs ``λe. get_read_args e = x``)
+  THENC (SIMP_CONV (srw_ss() ++ boolSimps.DNF_ss) [AC CONJ_ASSOC CONJ_COMM]) ;
+
+Theorem bir_get_stmt_bir_spinlock_prog_BirStmt_Generic =
+  EVAL ``bir_get_stmt bir_spinlock_prog x = BirStmt_Generic stm``
+  |> SIMP_RULE (srw_ss() ++ boolSimps.DNF_ss) [AllCaseEqs(),wordsTheory.NUMERAL_LESS_THM]
+  |> CONV_RULE CONJ_EQ_NEQ_conv
+  |> GEN_ALL
+
+Theorem bir_get_stmt_bir_spinlock_prog_BirStmt_Fence =
+  EVAL ``bir_get_stmt bir_spinlock_prog x = BirStmt_Fence mo1 mo2``
+  |> SIMP_RULE (srw_ss() ++ boolSimps.DNF_ss) [AllCaseEqs(),wordsTheory.NUMERAL_LESS_THM]
+  |> CONV_RULE CONJ_EQ_NEQ_conv
+  |> GEN_ALL
+
+Theorem bir_get_stmt_bir_spinlock_prog_BirStmt_Branch =
+  EVAL ``bir_get_stmt bir_spinlock_prog x = BirStmt_Branch a1 a2 a3``
+  |> SIMP_RULE (srw_ss() ++ boolSimps.DNF_ss) [AllCaseEqs(),wordsTheory.NUMERAL_LESS_THM]
+  |> CONV_RULE CONJ_EQ_NEQ_conv
+  |> GEN_ALL
+
+Theorem bir_get_stmt_bir_spinlock_prog_BirStmt_Expr =
+  EVAL ``bir_get_stmt bir_spinlock_prog x = BirStmt_Expr var e``
+  |> SIMP_RULE (srw_ss() ++ boolSimps.DNF_ss) [AllCaseEqs(),wordsTheory.NUMERAL_LESS_THM]
+  |> CONV_RULE CONJ_EQ_NEQ_conv
+  |> GEN_ALL
+
+(*
+bir_get_stmt_bir_spinlock_prog_BirStmt_Write_EQ
+bir_get_stmt_bir_spinlock_prog_BirStmt_Read_EQ
+*)
+
+Theorem bir_get_stmt_bir_spinlock_prog_BirStmt_Amo =
+  EVAL ``bir_get_stmt bir_spinlock_prog x = BirStmt_Amo var a_e v_e acq rel``
+  |> SIMP_RULE (srw_ss() ++ boolSimps.DNF_ss) [AllCaseEqs()]
+
+Theorem bir_get_stmt_bir_spinlock_prog_BirStmt_None =
+  EVAL ``bir_get_stmt bir_spinlock_prog x = BirStmt_None``
+  |> SIMP_RULE (srw_ss() ++ boolSimps.DNF_ss) [AllCaseEqs(),wordsTheory.NUMERAL_LESS_THM]
+  |> CONV_RULE CONJ_EQ_NEQ_conv
+  |> GEN_ALL
+
+Theorem bir_get_spinlock_stmts =
+  map (CONV_RULE (ONCE_DEPTH_CONV $ LHS_CONV SYM_CONV))
+      [bir_get_stmt_bir_spinlock_prog_BirStmt_Read_EQ,
+      bir_get_stmt_bir_spinlock_prog_BirStmt_Write_EQ,
+      bir_get_stmt_bir_spinlock_prog_BirStmt_Fence,
+      bir_get_stmt_bir_spinlock_prog_BirStmt_Generic,
+      bir_get_stmt_bir_spinlock_prog_BirStmt_Branch,
+      bir_get_stmt_bir_spinlock_prog_BirStmt_None,
+      bir_get_stmt_bir_spinlock_prog_BirStmt_Amo,
+      bir_get_stmt_bir_spinlock_prog_BirStmt_Expr]
+  |> LIST_CONJ
+
+Definition init1_def:
+  init1 st <=>
+    st.bst_pc = <| bpc_index := 0; bpc_label := BL_Address $ Imm64 0w |>
+End
+
+Definition init_def:
+  init cores =
+    !cid p st. FLOOKUP cores cid = SOME $ Core cid p st ==> init1 st
+End
+
+Theorem core_runs_spinlock_init1:
+  !cid cores. core_runs_spinlock cid cores
+  ==> ?st. FLOOKUP cores cid = SOME $ Core cid bir_spinlock_prog st /\ init1 st
+Proof
+  rw[init1_def,core_runs_spinlock_def,core_runs_prog_def]
+  >> fs[bir_programTheory.bir_state_init_def,bir_programTheory.bir_pc_first_def,bir_spinlock_prog_def,bir_programTheory.bir_block_pc_def,bir_program_labelsTheory.BL_Address_HC_def]
+QED
+
+Theorem cores_run_spinlock_init:
+  !tr. cores_run_spinlock $ FST $ HD tr ==> init $ FST $ HD tr
+Proof
+  rw[cores_run_spinlock_def,init_def]
+  >> res_tac
+  >> imp_res_tac core_runs_spinlock_init1
+  >> gs[]
+QED
+
+(*
+  all possible steps with the spinlock
+  sl_step (blck,pc) (blck',pc')
+*)
+Inductive sl_step:
+  sl_step (BL_Address $ Imm64 x,y) (BL_Address $ Imm64 x,y)
+  /\ sl_step (BL_Address $ Imm64 0w,0n) (BL_Address $ Imm64 0w,1)
+  /\ sl_step (BL_Address $ Imm64 0w,1)  (BL_Address $ Imm64 4w,0)
+  /\ sl_step (BL_Address $ Imm64 4w,0)  (BL_Address $ Imm64 4w,1)
+  /\ sl_step (BL_Address $ Imm64 4w,1)  (BL_Address $ Imm64 8w,0)
+  /\ sl_step (BL_Address $ Imm64 8w,0)  (BL_Address $ Imm64 8w,1)
+  /\ sl_step (BL_Address $ Imm64 8w,1)  (BL_Address $ Imm64 12w,0)
+  /\ sl_step (BL_Address $ Imm64 12w,0) (BL_Address $ Imm64 12w,1)
+  /\ sl_step (BL_Address $ Imm64 12w,1) (BL_Address $ Imm64 12w,3)
+  /\ sl_step (BL_Address $ Imm64 12w,3) (BL_Address $ Imm64 16w,0)
+  /\ sl_step (BL_Address $ Imm64 16w,0) (BL_Address $ Imm64 12w,0)
+  /\ sl_step (BL_Address $ Imm64 16w,0) (BL_Address $ Imm64 20w,0)
+  /\ sl_step (BL_Address $ Imm64 20w,0) (BL_Address $ Imm64 20w,1)
+  /\ sl_step (BL_Address $ Imm64 20w,1) (BL_Address $ Imm64 20w,2)
+  /\ sl_step (BL_Address $ Imm64 20w,2) (BL_Address $ Imm64 20w,5)
+  /\ sl_step (BL_Address $ Imm64 20w,5) (BL_Address $ Imm64 24w,0)
+  /\ sl_step (BL_Address $ Imm64 24w,0) (BL_Address $ Imm64 12w,0)
+  /\ sl_step (BL_Address $ Imm64 24w,0) (BL_Address $ Imm64 28w,0)
+End
+
+Definition bst_pc_tuple_def:
+  bst_pc_tuple x = (x.bpc_label,x.bpc_index)
+End
+
+(*
+(*
+  TODO make this a function taking a term:
+  val term = ``sl_step``
+ *)
+val fun_snd_imp =
+  let
+    val values =
+      map (rand o concl o SPEC_ALL) $ CONJUNCTS sl_step_rules
+    val term' =
+      mk_imp (``sl_step å1 å2``,
+        map (fn value => mk_eq (``å2:bir_label_t # num``, value)) values
+        |> list_mk_disj)
+  in
+   prove(term', dsimp[sl_step_cases])
+  end
+*)
+
+Definition reachable_pc_def:
+  reachable_pc pc <=>
+    !bpt. bpt = bst_pc_tuple pc ==>
+    bpt = (BL_Address $ Imm64 0w,1) \/ bpt = (BL_Address $ Imm64 4w,0) \/
+    bpt = (BL_Address $ Imm64 4w,1) \/ bpt = (BL_Address $ Imm64 8w,0) \/
+    bpt = (BL_Address $ Imm64 8w,1) \/ bpt = (BL_Address $ Imm64 12w,0) \/
+    bpt = (BL_Address $ Imm64 12w,1) \/ bpt = (BL_Address $ Imm64 12w,3) \/
+    bpt = (BL_Address $ Imm64 16w,0) \/ bpt = (BL_Address $ Imm64 20w,0) \/
+    bpt = (BL_Address $ Imm64 20w,1) \/ bpt = (BL_Address $ Imm64 20w,2) \/
+    bpt = (BL_Address $ Imm64 20w,5) \/ bpt = (BL_Address $ Imm64 24w,0) \/
+    bpt = (BL_Address $ Imm64 28w,0) \/ bpt = (BL_Address $ Imm64 0w,0)
+End
+
+Theorem reachable_pc_sl_step_imp:
+  !pc pc'. reachable_pc pc
+  /\ sl_step (bst_pc_tuple pc) (bst_pc_tuple pc')
+  ==> reachable_pc pc'
+Proof
+  rw[reachable_pc_def]
+  >> gvs[sl_step_cases]
+QED
+
+Theorem reachable_pc_sim:
+  !i tr cid p st st'. wf_trace tr
+  /\ SUC i < LENGTH tr
+  /\ core_runs_spinlock cid $ FST $ HD tr
+  /\ FLOOKUP (FST $ EL i tr) cid = SOME $ Core cid p st
+  /\ FLOOKUP (FST $ EL (SUC i) tr) cid = SOME $ Core cid p st'
+  /\ reachable_pc st.bst_pc
+  ==> sl_step (bst_pc_tuple st.bst_pc) (bst_pc_tuple st'.bst_pc)
+Proof
+  rpt gen_tac >> strip_tac
+  >> reverse $ Cases_on `parstep_nice cid (EL i tr) (EL (SUC i) tr)`
+  >- (
+    drule_all_then assume_tac wf_trace_NOT_parstep_nice_state_EQ'
+    >> fs[]
+    >> gvs[sl_step_rules,reachable_pc_def]
+  )
+  >> drule_all_then assume_tac wf_trace_core_runs_spinlock_FLOOKUP
+(* the remaining tactic mimick an EVAL for a parstep{_nice,} transition
+ * in the context of a concrete program 'bir_spinlock_prog'
+ * with the extracted possible pc locations of different instructions
+ * encoded in bir_get_stmt_bir_spinlock_prog_BirStmt_*
+ *)
+  >> fs[parstep_nice_def,parstep_cases,cstep_cases,FLOOKUP_UPDATE,clstep_cases,bir_programTheory.bir_pc_next_def,bst_pc_tuple_def,sl_step_cases]
+  >> gvs[FLOOKUP_UPDATE,bir_get_spinlock_stmts]
+  >> gvs[bir_programTheory.bir_pc_next_def,AllCaseEqs(),bir_get_stmt_bir_spinlock_prog_BirStmt_Write_EQ,bir_get_stmt_bir_spinlock_prog_BirStmt_Read_EQ,bir_get_stmt_bir_spinlock_prog_BirStmt_Expr,bir_get_stmt_bir_spinlock_prog_BirStmt_Generic,bir_get_stmt_bir_spinlock_prog_BirStmt_Expr,bir_get_stmt_bir_spinlock_prog_BirStmt_None,bir_get_stmt_bir_spinlock_prog_BirStmt_Branch,bir_programTheory.bir_exec_stmt_def,bir_programTheory.bir_exec_stmtB_def,bir_programTheory.bir_exec_stmt_assert_def,bir_expTheory.bir_eval_exp_def,bir_expTheory.bir_eval_bin_pred_def,bir_expTheory.bir_eval_bin_exp_def,bir_programTheory.bir_state_set_typeerror_def,bir_programTheory.bir_exec_stmtE_def,bir_programTheory.bir_exec_stmt_jmp_def,bir_programTheory.bir_eval_label_exp_def,bir_programTheory.bir_exec_stmt_jmp_to_label_def,bir_programTheory.bir_block_pc_def,bir_programTheory.bir_exec_stmt_cjmp_def,bst_pc_tuple_def,reachable_pc_def]
+  >> BasicProvers.every_case_tac
+  >> gvs[bir_programTheory.bir_pc_next_def,AllCaseEqs(),bir_get_stmt_bir_spinlock_prog_BirStmt_Write_EQ,bir_get_stmt_bir_spinlock_prog_BirStmt_Read_EQ,bir_get_stmt_bir_spinlock_prog_BirStmt_Expr,bir_get_stmt_bir_spinlock_prog_BirStmt_Generic,bir_get_stmt_bir_spinlock_prog_BirStmt_Expr,bir_get_stmt_bir_spinlock_prog_BirStmt_None,bir_get_stmt_bir_spinlock_prog_BirStmt_Branch,bir_programTheory.bir_exec_stmt_def,bir_programTheory.bir_exec_stmtB_def,bir_programTheory.bir_exec_stmt_assert_def,bir_expTheory.bir_eval_exp_def,bir_expTheory.bir_eval_bin_pred_def,bir_expTheory.bir_eval_bin_exp_def,bir_programTheory.bir_state_set_typeerror_def,bir_programTheory.bir_exec_stmtE_def,bir_programTheory.bir_exec_stmt_jmp_def,bir_programTheory.bir_eval_label_exp_def,bir_programTheory.bir_exec_stmt_jmp_to_label_def,bir_programTheory.bir_block_pc_def,get_fulfil_args_def,get_read_args_def]
+QED
+
+Theorem wf_trace_reachable_pc:
+  !i tr cid p st st'. wf_trace tr
+  /\ i < LENGTH tr
+  /\ core_runs_spinlock cid $ FST $ HD tr
+  /\ FLOOKUP (FST $ EL i tr) cid = SOME $ Core cid p st
+  ==> reachable_pc st.bst_pc
+Proof
+  Induct >> rpt strip_tac
+  >- (
+    imp_res_tac core_runs_spinlock_init1
+    >> gs[bst_pc_tuple_def,reachable_pc_def,init1_def]
+  )
+  >> rev_drule_all_then strip_assume_tac wf_trace_cid_backward1
+  >> first_x_assum $ drule_at_then (Pat `FLOOKUP _ _ = _`) assume_tac
+  >> gs[]
+  >> drule_all_then assume_tac reachable_pc_sim
+  >> dxrule_all reachable_pc_sl_step_imp
+  >> fs[]
+QED
+
+Theorem reachable_pc_sl_step:
+  !i tr cid p st st'. wf_trace tr
+  /\ SUC i < LENGTH tr
+  /\ core_runs_spinlock cid $ FST $ HD tr
+  /\ FLOOKUP (FST $ EL i tr) cid = SOME $ Core cid p st
+  /\ FLOOKUP (FST $ EL (SUC i) tr) cid = SOME $ Core cid p st'
+  ==> reachable_pc st.bst_pc
+    /\ reachable_pc st'.bst_pc
+    /\ sl_step (bst_pc_tuple st.bst_pc) (bst_pc_tuple st'.bst_pc)
+Proof
+  rpt gen_tac >> strip_tac
+  >> rev_drule_at_then (Pat `FLOOKUP _ _ = _`) assume_tac wf_trace_reachable_pc
+  >> drule_at_then (Pat `FLOOKUP _ _ = _`) assume_tac wf_trace_reachable_pc
+  >> gs[]
+  >> rev_drule_all_then irule reachable_pc_sim
+QED
+
+Theorem bir_env_def_spinlock =
+  EVAL ``bir_env_default $ bir_envty_of_vs $ bir_varset_of_program bir_spinlock_prog``
+  |> SIMP_RULE (srw_ss()) [PULL_FORALL,bir_valuesTheory.bir_default_value_of_type_def,combinTheory.o_DEF,pred_setTheory.DIFF_DEF,bir_envTheory.bir_var_type_def,COND_RAND]
+
+(* unique properties *)
+
+Definition unique_def:
+  unique fmap P =
+    !id id' x x'. FLOOKUP fmap id = SOME x /\ P x
+      /\ FLOOKUP fmap id' = SOME x' /\ P x'
+      ==> id = id'
+End
+
+Theorem FLOOKUP_NOT_unique_eq:
+  !P cores cid st st'. FLOOKUP cores cid = SOME st
+  /\ ~(P st) /\ ~(P st')
+  ==> unique (FUPDATE cores (cid,st')) P = unique cores P
+Proof
+  rw[unique_def,EQ_IMP_THM]
+  >- (
+    first_x_assum irule
+    >> dsimp[FLOOKUP_UPDATE,AllCaseEqs()]
+    >> conj_tac >> spose_not_then assume_tac >> gvs[]
+  )
+  >> gs[FLOOKUP_UPDATE,AllCaseEqs()]
+QED
+
+Theorem FLOOKUP_unique_eq:
+  FLOOKUP cores cid = SOME st
+  /\ P st /\ P st'
+  ==> unique (FUPDATE cores (cid,st')) P = unique cores P
+Proof
+  rw[unique_def,EQ_IMP_THM]
+  >- (
+    first_x_assum irule
+    >> dsimp[FLOOKUP_UPDATE,AllCaseEqs(),LEFT_AND_OVER_OR,RIGHT_AND_OVER_OR]
+    >> metis_tac[]
+  )
+  >> gs[FLOOKUP_UPDATE,AllCaseEqs()]
+QED
+
+(* invariant *)
+
+Definition in_crit_def:
+  in_crit (Core id p st) <=>
+    st.bst_pc = <|bpc_label := BL_Address (Imm64 28w); bpc_index := 0|>
+End
+
+Theorem in_crit_sl_step:
+  !cid p st st'.
+  sl_step (bst_pc_tuple st.bst_pc) (bst_pc_tuple st'.bst_pc)
+  /\ st.bst_pc <> st'.bst_pc
+  /\ ~(in_crit $ Core cid p st')
+  ==> ~(in_crit $ Core cid p st)
+Proof
+  rw[sl_step_cases,in_crit_def,bst_pc_tuple_def,bir_programTheory.bir_programcounter_t_component_equality]
+  >> gvs[]
+QED
+
+Theorem in_crit_reachable_pc:
+  in_crit $ Core cid p st
+  ==> reachable_pc st.bst_pc
+Proof
+  fs[in_crit_def,reachable_pc_def,bst_pc_tuple_def]
+QED
+
+Definition invariant_def:
+  invariant cores = unique cores in_crit
+End
+
+Theorem init_unique_in_crit_imp:
+  !i tr. wf_trace tr /\ wf_trace1 tr
+  /\ init (FST $ HD tr)
+  ==> invariant (FST $ HD tr)
+Proof
+  rw[init1_def,init_def,invariant_def,unique_def,Excl"EL",GSYM EL,Excl"EL_restricted"]
+  >> drule_then drule wf_trace1_FLOOKUP
+  >> drule_then rev_drule wf_trace1_FLOOKUP
+  >> rw[wf_trace_NOT_NULL,LENGTH_NOT_NULL]
+  >> fs[in_crit_def]
+  >> qpat_x_assum `!cid p st. FLOOKUP _ _ = _ ==> _` imp_res_tac
+  >> gs[]
+QED
+
+(* no loops in the spinlock program *)
+
+val pc_inc_tac =
+  spose_not_then kall_tac
+  >> fs[bir_programTheory.bir_state_t_component_equality,bir_programTheory.bir_programcounter_t_component_equality]
+  >> rpt $ qpat_x_assum `_.bst_pc.bpc_label = _` mp_tac
+  >> rpt $ qpat_x_assum `_.bst_pc.bpc_index = _` mp_tac
+  >> rpt $ first_x_assum kall_tac
+  >> rpt strip_tac
+  >> BasicProvers.every_case_tac
+  >> fs[bir_programTheory.bir_pc_next_def] ;
+
+Theorem parstep_sl_step_progress:
+  !tr i cid p st st'. wf_trace tr
+  /\ SUC i < LENGTH tr
+  /\ progressing_trace tr
+  /\ core_runs_spinlock cid $ FST $ HD tr
+  /\ parstep_nice cid (EL i tr) (EL (SUC i) tr)
+  /\ FLOOKUP (FST $ EL i tr) cid = SOME (Core cid p st)
+  /\ FLOOKUP (FST $ EL (SUC i) tr) cid = SOME (Core cid p st')
+  /\ sl_step (bst_pc_tuple st.bst_pc) (bst_pc_tuple st'.bst_pc)
+  /\ ~is_promise cid (LENGTH (SND (EL i tr)) + 1) (EL i tr) (EL (SUC i) tr)
+  ==> st.bst_pc <> st'.bst_pc
+Proof
+  rpt gen_tac >> strip_tac
+  >> fs[progressing_trace_def,progressing_def]
+  >> first_x_assum $ drule_then drule
+  >> drule_all_then assume_tac wf_trace_core_runs_spinlock_FLOOKUP
+  >> reverse $ gvs[parstep_nice_def,parstep_cases,cstep_cases,FLOOKUP_UPDATE]
+  >- gs[is_promise_def,FLOOKUP_UPDATE,bir_promisingTheory.mem_msg_t_component_equality]
+  >> PRED_ASSUM is_neg kall_tac
+  >> fs[Once MONO_NOT_EQ] >> strip_tac
+  >> drule wf_trace_reachable_pc
+  >> rpt $ disch_then drule
+  >> disch_then assume_tac
+  >> fs[clstep_cases]
+  >- pc_inc_tac
+  >- pc_inc_tac
+  >- pc_inc_tac
+  >- pc_inc_tac
+  >- pc_inc_tac
+  >- (
+    (* branch *)
+    gvs[bir_get_stmt_bir_spinlock_prog_BirStmt_Branch,FLOOKUP_UPDATE]
+    >> cheat
+  )
+  >- pc_inc_tac
+  >- (
+    gvs[FLOOKUP_UPDATE]
+    >> spose_not_then kall_tac
+    >> gvs[bir_get_stmt_bir_spinlock_prog_BirStmt_Generic,FLOOKUP_UPDATE,bir_programTheory.bir_state_t_component_equality,bir_programTheory.bir_programcounter_t_component_equality]
+    >> cheat (* evaluate statements that change the pc *)
+  )
+QED
+
+(* no promises possible after a certain program counter *)
+(* TODO *)
+
+Theorem core_runs_spinlock_fulfils:
+  !tr i cid p st st' t. wf_trace tr
+  /\ SUC i < LENGTH tr
+  /\ progressing_trace tr
+  /\ core_runs_spinlock cid $ FST $ HD tr
+  /\ is_fulfil cid t (EL i tr) (FST $ EL (SUC i) tr)
+  /\ FLOOKUP (FST $ EL i tr) cid = SOME $ Core cid p st
+  /\ FLOOKUP (FST $ EL (SUC i) tr) cid = SOME $ Core cid p st'
+  ==>
+      (bst_pc_tuple st.bst_pc = (BL_Address (Imm64 12w),2)
+      /\ bst_pc_tuple st'.bst_pc = (BL_Address (Imm64 12w),3))
+      (* ~rel ~acq ~xcl, loc = ...*)
+    \/ (
+     bst_pc_tuple st.bst_pc = (BL_Address (Imm64 20w),2)
+     /\ bst_pc_tuple st'.bst_pc = (BL_Address (Imm64 20w),5)
+      (* ~rel ~acq xcl, loc = ...*)
+      (* bir_eval_exp_view (BExp_Den spinlock_var) s.bst_environ s.bst_viewenv *)
+    )
+Proof
+  rpt strip_tac
+  >> drule_all_then assume_tac wf_trace_core_runs_spinlock_FLOOKUP
+  >> drule_all_then strip_assume_tac is_fulfil_parstep_nice_eq
+  >> gvs[FLOOKUP_UPDATE,bir_get_stmt_bir_spinlock_prog_BirStmt_Write_EQ,bst_pc_tuple_def,bir_programTheory.bir_pc_next_def]
+QED
+
+(*
+Theorem in_crit_before4:
+  !tr i cid p st x.
+  wf_trace tr /\ i < LENGTH tr
+  /\ progressing_trace tr
+  /\ core_runs_spinlock cid $ FST $ HD tr
+  /\ FLOOKUP (FST (EL i tr)) cid = SOME (Core cid p st)
+  /\ bst_pc_tuple st.bst_pc = (BL_Address (Imm64 20w),2)
+  ==> ?j st' t. j < i
+     /\ parstep_nice cid (EL j tr) (EL (SUC j) tr)
+     /\ same_state_prop_range cid tr (SUC j) i I
+     /\ ~is_promise cid (LENGTH (SND (EL j tr)) + 1) (EL j tr) (EL (SUC j) tr)
+     /\ FLOOKUP (FST (EL j tr)) cid = SOME (Core cid p st')
+     /\ FLOOKUP (FST (EL (SUC j) tr)) cid = SOME (Core cid p st)
+     /\ bst_pc_tuple st'.bst_pc = (BL_Address (Imm64 20w),1)
+     /\ st'.bst_environ = st.bst_environ
+Proof
+  rpt strip_tac
+  >> drule_all_then strip_assume_tac previous_state_change
+  >- (
+    drule core_runs_spinlock_NOT_init_pc
+    >> rpt $ disch_then $ drule_at Any
+    >> fs[init1_def,bir_programTheory.bir_state_t_component_equality,bir_programTheory.bir_programcounter_t_component_equality,bst_pc_tuple_def]
+  )
+  >> Cases_on `i` >> fs[]
+  >> Cases_on `is_promise cid (LENGTH (SND (EL j tr)) + 1) (EL j tr) (EL (SUC j) tr)`
+  >- (
+    cheat (* any such new promise cannot be fulfiled *)
+  )
+  >> drule_all_then assume_tac same_state_prop_indexes
+  >> drule_at (Pat `FLOOKUP _ _ = _`)  wf_trace_cid_backward
+  >> disch_then (fn thm =>
+    qspec_then `j` assume_tac thm
+    >> qspec_then `SUC j` assume_tac thm)
+  >> gvs[same_state_prop_def]
+  >> qhdtm_assum `parstep_nice` $ irule_at Any
+  >> fs[]
+  >> drule_at_then (Pat `parstep_nice _ _ _`) assume_tac parstep_sl_step_progress
+  >> drule_at_then (Pat `FLOOKUP (FST $ EL (SUC _) _) _ = _`) assume_tac reachable_pc_sl_step
+  >> gs[GSYM PULL_EXISTS]
+  >> qpat_x_assum `reachable_pc st.bst_pc` kall_tac
+  >> conj_asm1_tac
+  >- gs[sl_step_cases,in_crit_def,bst_pc_tuple_def,bir_programTheory.bir_programcounter_t_component_equality]
+  >> conj_asm1_tac
+  >- (
+    fs[bir_get_stmt_bir_spinlock_prog_BirStmt_Write_EQ,bst_pc_tuple_def,bir_programTheory.bir_programcounter_t_component_equality,spinlock_var_def,bir_promisingTheory.is_amo_def,bir_get_program_block_info_by_label']
+(*
+   alternatively:
+   EVAL_TAC >> fs[bst_pc_tuple_def,get_read_args_def,get_fulfil_args_def]
+*)
+  )
+  >> qhdtm_x_assum `sl_step` kall_tac
+  >> qhdtm_x_assum `reachable_pc` kall_tac
+  >> drule_all_then assume_tac wf_trace_core_runs_spinlock_FLOOKUP
+  >> gvs[is_fulfil_xcl_def,parstep_nice_def,parstep_cases,FLOOKUP_UPDATE,cstep_cases,clstep_cases]
+  >- (
+    (* the exclusive write is successful *)
+    drule_all_then assume_tac xclfail_update_envs
+    >> Cases_on `st''.bst_environ`
+    >> gvs[bir_programTheory.bir_pc_next_def,bst_pc_tuple_def,bir_programTheory.bir_programcounter_t_component_equality,bir_envTheory.bir_env_update_def,bir_envTheory.bir_var_name_def,bir_envTheory.bir_var_type_def]
+    >> qpat_x_assum `bir_eval_unary_exp _ _ = _` mp_tac
+    >> EVAL_TAC >> strip_tac
+    >> fs[bir_valuesTheory.bir_dest_bool_val_def]
+  )
+  >> qpat_assum `MEM _ _` $ irule_at Any
+  >> fs[PRE_SUB1,oEL_THM]
+  >> spose_not_then assume_tac
+  >> fs[bir_get_stmt_write,fulfil_atomic_ok_def]
+QED
+*)
+
+(* a core with a non-initial pc has progressed *)
+
+Theorem core_runs_spinlock_NOT_init_pc:
+  !tr i cid p st. wf_trace tr
+  /\ i < LENGTH tr
+  /\ progressing_trace tr
+  /\ core_runs_spinlock cid $ FST $ HD tr
+  /\ FLOOKUP (FST $ EL i tr) cid = SOME $ Core cid p st
+  /\ ~init1 st
+  ==> ~same_state_prop_range cid tr 0 i I
+Proof
+  rpt strip_tac
+  >> drule_all_then assume_tac same_state_prop_indexes
+  >> drule_all_then assume_tac core_runs_spinlock_init1
+  >> drule_at_then (Pat `FLOOKUP _ _ = _`) (qspec_then `0` assume_tac) wf_trace_cid_backward
+  >> gs[same_state_prop_def]
+QED
+
+Theorem xclfail_update_envs:
+  !new_viewenv new_env st.
+  bst_pc_tuple st.bst_pc = (BL_Address (Imm64 20w),2)
+  /\ SOME new_viewenv = xclfail_update_viewenv bir_spinlock_prog st
+  /\ SOME new_env = xclfail_update_env bir_spinlock_prog st
+  ==> new_viewenv = st.bst_viewenv |+ (BVar "x6" (BType_Imm Bit64),0) /\
+    SOME new_env = bir_env_update (bir_var_name (BVar "x6" (BType_Imm Bit64)))
+      (BVal_Imm (Imm64 1w)) (bir_var_type (BVar "x6" (BType_Imm Bit64)))
+      st.bst_environ
+Proof
+  rpt gen_tac
+  >> fs[GSYM AND_IMP_INTRO]
+  >> strip_tac
+  >> EVAL_TAC
+  >> fs[bst_pc_tuple_def,bir_envTheory.bir_var_name_def,bir_envTheory.bir_var_type_def]
+QED
+
+Theorem in_crit_before3:
+  !tr i cid p st x.
+  wf_trace tr /\ i < LENGTH tr
+  /\ progressing_trace tr
+  /\ core_runs_spinlock cid $ FST $ HD tr
+  /\ FLOOKUP (FST (EL i tr)) cid = SOME (Core cid p st)
+  /\ bst_pc_tuple st.bst_pc = (BL_Address (Imm64 20w),5)
+  /\ bir_eval_unary_exp BIExp_Not
+    (bir_eval_bin_pred BIExp_Equal
+      (bir_env_read (BVar "x6" (BType_Imm Bit64)) st.bst_environ)
+      (SOME (BVal_Imm (Imm64 0w)))) = SOME x
+  /\ bir_dest_bool_val x = SOME F
+  ==> ?j st' t. j < i
+     /\ parstep_nice cid (EL j tr) (EL (SUC j) tr)
+     /\ same_state_prop_range cid tr (SUC j) i I
+     /\ ~is_promise cid (LENGTH (SND (EL j tr)) + 1) (EL j tr) (EL (SUC j) tr)
+     /\ FLOOKUP (FST (EL j tr)) cid = SOME (Core cid p st')
+     /\ FLOOKUP (FST (EL (SUC j) tr)) cid = SOME (Core cid p st)
+     /\ bst_pc_tuple st'.bst_pc = (BL_Address (Imm64 20w),2)
+     /\ bir_get_stmt (bir_spinlock_prog :string bir_program_t) st'.bst_pc =
+        BirStmt_Write (BExp_Den (BVar "x7" (BType_Imm Bit64)))
+          (BExp_Cast BIExp_LowCast (BExp_Const (Imm64 0w)) Bit32) T F F
+     /\ is_fulfil_xcl cid t (EL j tr) (FST $ EL (SUC j) tr)
+     /\ t < LENGTH (SND $ EL j tr) + 1
+     /\ (EL (PRE t) (SND $ EL j tr)).cid = cid
+Proof
+  rpt strip_tac
+  >> drule_all_then strip_assume_tac previous_state_change
+  >- (
+    drule core_runs_spinlock_NOT_init_pc
+    >> rpt $ disch_then $ drule_at Any
+    >> fs[init1_def,bir_programTheory.bir_state_t_component_equality,bir_programTheory.bir_programcounter_t_component_equality,bst_pc_tuple_def]
+  )
+  >> Cases_on `i` >> fs[]
+  >> Cases_on `is_promise cid (LENGTH (SND (EL j tr)) + 1) (EL j tr) (EL (SUC j) tr)`
+  >- (
+    cheat (* any such new promise cannot be fulfiled *)
+  )
+  >> drule_all_then assume_tac same_state_prop_indexes
+  >> drule_at (Pat `FLOOKUP _ _ = _`)  wf_trace_cid_backward
+  >> disch_then (fn thm =>
+    qspec_then `j` assume_tac thm
+    >> qspec_then `SUC j` assume_tac thm)
+  >> gvs[same_state_prop_def]
+  >> qhdtm_assum `parstep_nice` $ irule_at Any
+  >> fs[]
+  >> drule_at_then (Pat `parstep_nice _ _ _`) assume_tac parstep_sl_step_progress
+  >> drule_at_then (Pat `FLOOKUP (FST $ EL (SUC _) _) _ = _`) assume_tac reachable_pc_sl_step
+  >> gs[GSYM PULL_EXISTS]
+  >> qpat_x_assum `reachable_pc st.bst_pc` kall_tac
+  >> conj_asm1_tac
+  >- gs[sl_step_cases,in_crit_def,bst_pc_tuple_def,bir_programTheory.bir_programcounter_t_component_equality]
+  >> conj_asm1_tac
+  >- (
+    fs[bir_get_stmt_bir_spinlock_prog_BirStmt_Write_EQ,bst_pc_tuple_def,bir_programTheory.bir_programcounter_t_component_equality,spinlock_var_def,bir_promisingTheory.is_amo_def,bir_get_program_block_info_by_label']
+(*
+   alternatively:
+   EVAL_TAC >> fs[bst_pc_tuple_def,get_read_args_def,get_fulfil_args_def]
+*)
+  )
+  >> qhdtm_x_assum `sl_step` kall_tac
+  >> qhdtm_x_assum `reachable_pc` kall_tac
+  >> drule_all_then assume_tac wf_trace_core_runs_spinlock_FLOOKUP
+  >> gvs[is_fulfil_xcl_def,parstep_nice_def,parstep_cases,FLOOKUP_UPDATE,cstep_cases,clstep_cases]
+  >- (
+    (* the exclusive write is successful *)
+    drule_all_then assume_tac xclfail_update_envs
+    >> Cases_on `st''.bst_environ`
+    >> gvs[bir_programTheory.bir_pc_next_def,bst_pc_tuple_def,bir_programTheory.bir_programcounter_t_component_equality,bir_envTheory.bir_env_update_def,bir_envTheory.bir_var_name_def,bir_envTheory.bir_var_type_def]
+    >> qpat_x_assum `bir_eval_unary_exp _ _ = _` mp_tac
+    >> EVAL_TAC >> strip_tac
+    >> fs[bir_valuesTheory.bir_dest_bool_val_def]
+  )
+  >> qpat_assum `MEM _ _` $ irule_at Any
+  >> fs[PRE_SUB1,oEL_THM]
+  >> spose_not_then assume_tac
+  >> fs[bir_get_stmt_write,fulfil_atomic_ok_def]
+QED
+
+Theorem in_crit_before2:
+  !tr i cid p st x.
+  wf_trace tr /\ i < LENGTH tr
+  /\ progressing_trace tr
+  /\ core_runs_spinlock cid $ FST $ HD tr
+  /\ FLOOKUP (FST (EL i tr)) cid = SOME (Core cid p st)
+  /\ bst_pc_tuple st.bst_pc = (BL_Address (Imm64 24w),0)
+  ==> ?j st'. j < i
+    /\ parstep_nice cid (EL j tr) (EL (SUC j) tr)
+    /\ same_state_prop_range cid tr (SUC j) i I
+    /\ ~is_promise cid (LENGTH (SND (EL j tr)) + 1) (EL j tr) (EL (SUC j) tr)
+    /\ FLOOKUP (FST (EL j tr)) cid = SOME (Core cid p st')
+    /\ FLOOKUP (FST (EL (SUC j) tr)) cid = SOME (Core cid p st)
+    /\ bst_pc_tuple st'.bst_pc = (BL_Address (Imm64 20w),5)
+    /\ st.bst_environ = st'.bst_environ
+Proof
+  rpt strip_tac
+  >> drule_all_then strip_assume_tac previous_state_change
+  >- (
+    drule core_runs_spinlock_NOT_init_pc
+    >> rpt $ disch_then $ drule_at Any
+    >> fs[init1_def,bir_programTheory.bir_state_t_component_equality,bir_programTheory.bir_programcounter_t_component_equality,bst_pc_tuple_def]
+  )
+  >> Cases_on `i` >> fs[]
+  >> Cases_on `is_promise cid (LENGTH (SND (EL j tr)) + 1) (EL j tr) (EL (SUC j) tr)`
+  >- (
+    cheat (* any such new promise cannot be fulfiled *)
+  )
+  >> drule_all_then assume_tac same_state_prop_indexes
+  >> drule_at (Pat `FLOOKUP _ _ = _`)  wf_trace_cid_backward
+  >> disch_then (fn thm =>
+    qspec_then `j` assume_tac thm
+    >> qspec_then `SUC j` assume_tac thm)
+  >> gvs[same_state_prop_def]
+  >> qhdtm_assum `parstep_nice` $ irule_at Any
+  >> fs[]
+  >> drule_at_then (Pat `parstep_nice _ _ _`) assume_tac parstep_sl_step_progress
+  >> drule_at_then (Pat `FLOOKUP (FST $ EL (SUC _) _) _ = _`) assume_tac reachable_pc_sl_step
+  >> gs[]
+  >> qpat_x_assum `reachable_pc st.bst_pc` kall_tac
+  >> conj_asm1_tac
+  >- gs[sl_step_cases,in_crit_def,bst_pc_tuple_def,bir_programTheory.bir_programcounter_t_component_equality]
+  >> `bir_get_stmt (bir_spinlock_prog :string bir_program_t) st''.bst_pc =
+        BirStmt_Generic
+          (BStmtE (BStmt_Jmp (BLE_Label (BL_Address (Imm64 24w)))))`
+    by fs[bir_get_stmt_bir_spinlock_prog_BirStmt_Generic,bst_pc_tuple_def]
+  >> qhdtm_x_assum `sl_step` kall_tac
+  >> qhdtm_x_assum `reachable_pc` kall_tac
+  >> drule_all_then assume_tac wf_trace_core_runs_spinlock_FLOOKUP
+  >> gvs[parstep_nice_def,parstep_cases,cstep_cases,clstep_cases,FLOOKUP_UPDATE]
+  >> gvs[bir_programTheory.bir_exec_stmt_def,bir_programTheory.bir_exec_stmtB_def,bir_programTheory.bir_exec_stmt_assert_def,bir_expTheory.bir_eval_exp_def,bir_expTheory.bir_eval_bin_pred_def,bir_expTheory.bir_eval_bin_exp_def,bir_programTheory.bir_state_set_typeerror_def,bir_programTheory.bir_exec_stmtE_def,bir_programTheory.bir_exec_stmt_jmp_def,bir_programTheory.bir_eval_label_exp_def,bir_programTheory.bir_exec_stmt_jmp_to_label_def,bir_programTheory.bir_block_pc_def,bir_programTheory.bir_exec_stmt_cjmp_def,bst_pc_tuple_def]
+  >> BasicProvers.every_case_tac
+  >> gs[bir_programTheory.bir_programcounter_t_component_equality,CaseEq"option"]
+QED
+
+(* properties about the step before entering in_crit *)
+
+Theorem in_crit_before1:
+  !tr i cid p st.
+  wf_trace tr /\ i < LENGTH tr
+  /\ progressing_trace tr
+  /\ core_runs_spinlock cid $ FST $ HD tr
+  /\ FLOOKUP (FST (EL i tr)) cid = SOME (Core cid p st)
+  /\ in_crit (Core cid p st)
+  ==> ?j st' x. j < i
+    /\ parstep_nice cid (EL j tr) (EL (SUC j) tr)
+    /\ same_state_prop_range cid tr (SUC j) i I
+    /\ ~is_promise cid (LENGTH (SND (EL j tr)) + 1) (EL j tr) (EL (SUC j) tr)
+    /\ FLOOKUP (FST (EL j tr)) cid = SOME (Core cid p st')
+    /\ FLOOKUP (FST (EL (SUC j) tr)) cid = SOME (Core cid p st)
+    /\ bst_pc_tuple st'.bst_pc = (BL_Address (Imm64 24w),0)
+    /\ bir_eval_unary_exp BIExp_Not
+      (bir_eval_bin_pred BIExp_Equal
+        (bir_env_read (BVar "x6" (BType_Imm Bit64)) st'.bst_environ)
+        (SOME (BVal_Imm (Imm64 0w)))) = SOME x
+    /\ bir_dest_bool_val x = SOME F
+Proof
+  rpt strip_tac
+  >> drule_all_then strip_assume_tac previous_state_change
+  >- (
+    drule core_runs_spinlock_NOT_init_pc
+    >> rpt $ disch_then $ drule_at Any
+    >> fs[init1_def,bir_programTheory.bir_state_t_component_equality,bir_programTheory.bir_programcounter_t_component_equality,bst_pc_tuple_def,in_crit_def]
+  )
+  >> Cases_on `i` >> fs[]
+  >> Cases_on `is_promise cid (LENGTH (SND (EL j tr)) + 1) (EL j tr) (EL (SUC j) tr)`
+  >- (
+    cheat (* any such new promise cannot be fulfiled *)
+  )
+  >> drule_all_then assume_tac same_state_prop_indexes
+  >> drule_at (Pat `FLOOKUP _ _ = _`)  wf_trace_cid_backward
+  >> disch_then (fn thm =>
+    qspec_then `j` assume_tac thm
+    >> qspec_then `SUC j` assume_tac thm)
+  >> gvs[same_state_prop_def]
+  >> qhdtm_assum `parstep_nice` $ irule_at Any
+  >> fs[]
+  >> drule_at_then (Pat `parstep_nice _ _ _`) assume_tac parstep_sl_step_progress
+  >> drule_at_then (Pat `FLOOKUP (FST $ EL (SUC _) _) _ = _`) assume_tac reachable_pc_sl_step
+  >> gs[GSYM PULL_EXISTS]
+  >> qpat_x_assum `reachable_pc st.bst_pc` kall_tac
+  >> conj_asm1_tac
+  >- gs[sl_step_cases,in_crit_def,bst_pc_tuple_def,bir_programTheory.bir_programcounter_t_component_equality]
+  >> `bir_get_stmt (bir_spinlock_prog :string bir_program_t) st''.bst_pc = BirStmt_Branch
+    (BExp_UnaryExp BIExp_Not
+      (BExp_BinPred BIExp_Equal
+          (BExp_Den $ BVar "x6" $ BType_Imm Bit64)
+          $ BExp_Const $ Imm64 0w))
+    (BLE_Label $ BL_Address $ Imm64 12w)
+    $ BLE_Label $ BL_Address $ Imm64 28w`
+    by fs[bir_get_stmt_bir_spinlock_prog_BirStmt_Branch,bst_pc_tuple_def]
+  >> qhdtm_x_assum `sl_step` kall_tac
+  >> qhdtm_x_assum `reachable_pc` kall_tac
+  >> drule_all_then assume_tac wf_trace_core_runs_spinlock_FLOOKUP
+  >> gvs[parstep_nice_def,parstep_cases,cstep_cases,clstep_cases,FLOOKUP_UPDATE]
+  >> gvs[bir_programTheory.bir_exec_stmt_def,bir_programTheory.bir_exec_stmtB_def,bir_programTheory.bir_exec_stmt_assert_def,bir_expTheory.bir_eval_exp_def,bir_expTheory.bir_eval_bin_pred_def,bir_expTheory.bir_eval_bin_exp_def,bir_programTheory.bir_state_set_typeerror_def,bir_programTheory.bir_exec_stmtE_def,bir_programTheory.bir_exec_stmt_jmp_def,bir_programTheory.bir_eval_label_exp_def,bir_programTheory.bir_exec_stmt_jmp_to_label_def,bir_programTheory.bir_block_pc_def,bir_programTheory.bir_exec_stmt_cjmp_def,bst_pc_tuple_def,in_crit_def]
+  >> BasicProvers.every_case_tac
+  >> gs[bir_programTheory.bir_programcounter_t_component_equality,CaseEq"option"]
+QED
+
+(* a core in the critical section has executed a successful exclusive fulfil *)
+
+Theorem in_crit_is_fulfil_xcl:
+  !tr i cid p st.
+  wf_trace tr /\ i < LENGTH tr
+  /\ progressing_trace tr
+  /\ core_runs_spinlock cid $ FST $ HD tr
+  /\ FLOOKUP (FST (EL i tr)) cid = SOME (Core cid p st)
+  /\ in_crit (Core cid p st)
+  ==> ?j t. j < i
+    /\ is_fulfil_xcl cid t (EL j tr) (FST $ EL (SUC j) tr)
+     /\ t < LENGTH (SND $ EL j tr) + 1
+     /\ cid = (EL (PRE t) (SND $ EL j tr)).cid
+Proof
+  rpt strip_tac
+  >> drule_all_then strip_assume_tac in_crit_before1
+  >> drule_at (Pat `bst_pc_tuple _ = _`) in_crit_before2
+  >> disch_then $ drule_at_then (Pat `FLOOKUP _ _ = _`) assume_tac
+  >> gs[]
+  >> drule_at (Pat `bst_pc_tuple _ = _`) in_crit_before3
+  >> disch_then $ drule_at_then (Pat `FLOOKUP _ _ = _`) assume_tac
+  >> gs[]
+  >> goal_assum $ drule_at $ Pat `is_fulfil_xcl _ _ _ _`
+  >> fs[]
+QED
+
+Theorem is_fulfil_xcl_bst_xclb_less_timestamp:
+  !tr i cid p st t. wf_trace tr /\ SUC i < LENGTH tr
+  /\ progressing_trace tr
+  /\ is_fulfil_xcl cid t (EL i tr) (FST $ EL (SUC i) tr)
+  /\ FLOOKUP (FST $ EL i tr) cid = SOME $ Core cid p st
+  ==> IS_SOME st.bst_xclb /\ (THE st.bst_xclb).xclb_view < t
+Proof
+  rpt gen_tac >> strip_tac
+  >> drule_all_then strip_assume_tac is_fulfil_xcl_is_fulfil
+  >> dxrule_at_then (Pat `is_fulfil _ _ _ _`) assume_tac is_fulfil_parstep_nice_eq
+  >> gvs[FLOOKUP_UPDATE,is_fulfil_xcl_def,get_xclb_view_def,optionTheory.IS_SOME_EXISTS]
+QED
+
+Theorem bst_fwdb_init:
+  !l cores cid p st.
+  FLOOKUP cores cid = SOME $ Core cid p st
+  /\ core_runs_spinlock cid cores
+  ==> st.bst_fwdb l = <|fwdb_time := 0; fwdb_view := 0; fwdb_xcl := F|>
+Proof
+  EVAL_TAC >> rpt strip_tac
+  >> gvs[]
+QED
+
+Theorem parstep_nice_NOT_is_fulfil_bst_fwdb_eq:
+  !tr i cid p st st' t.
+  wf_trace tr /\ SUC i < LENGTH tr
+  /\ progressing_trace tr
+  /\ parstep_nice cid (EL i tr) (EL (SUC i) tr)
+  /\ FLOOKUP (FST $ EL i tr) cid = SOME $ Core cid p st
+  /\ FLOOKUP (FST $ EL (SUC i) tr) cid = SOME $ Core cid p st'
+  /\ (!t. ~is_fulfil cid t (EL i tr) (FST $ EL (SUC i) tr))
+  /\ (!t. ~is_amo cid t (EL i tr) (FST $ EL (SUC i) tr))
+  ==> st.bst_fwdb = st'.bst_fwdb
+Proof
+  rpt strip_tac
+  >> gvs[parstep_nice_def,parstep_cases,FLOOKUP_UPDATE,cstep_cases,clstep_cases]
+  >- (
+    qmatch_asmsub_rename_tac `oEL (v_post - 1) (SND (EL i tr))`
+    >> qpat_x_assum `!t. ~is_fulfil _ t _ _` $ qspec_then `v_post` assume_tac
+    >> gvs[is_fulfil_def,FLOOKUP_UPDATE,bir_get_stmt_write,PRE_SUB1,oEL_THM]
+  )
+  >- (
+    qmatch_asmsub_rename_tac `oEL (v_post - 1) (SND (EL i tr))`
+    >> qpat_x_assum `!t. ~is_amo _ t _ _` $ qspec_then `v_post` assume_tac
+    >> gvs[is_amo_def,FLOOKUP_UPDATE,bir_get_stmt_write,PRE_SUB1,oEL_THM]
+  )
+  >- gvs[bir_programTheory.bir_exec_stmt_def,bir_programTheory.bir_exec_stmtE_def,bir_programTheory.bir_exec_stmt_cjmp_def,CaseEq"option",bir_programTheory.bir_exec_stmt_jmp_def,bir_programTheory.bir_state_set_typeerror_def,bir_programTheory.bir_exec_stmt_jmp_to_label_def,bir_get_stmt_branch,AllCaseEqs(),PRE_SUB1]
+  >- (
+    qmatch_assum_rename_tac `bir_get_stmt p _ = BirStmt_Generic stm`
+    >> Cases_on `stm`
+    >> gvs[bir_programTheory.bir_exec_stmt_def,bir_programTheory.bir_exec_stmtE_def,bir_programTheory.bir_exec_stmt_cjmp_def,CaseEq"option",bir_programTheory.bir_exec_stmt_jmp_def,bir_programTheory.bir_state_set_typeerror_def,bir_programTheory.bir_exec_stmt_jmp_to_label_def,bir_get_stmt_branch,AllCaseEqs(),pairTheory.ELIM_UNCURRY]
+    >> TRY (
+      qmatch_assum_rename_tac `bir_get_stmt p _ = BirStmt_Generic $ BStmtB b`
+      >> Cases_on `b`
+      >> gvs[bir_programTheory.bir_exec_stmt_def,bir_programTheory.bir_exec_stmtE_def,bir_programTheory.bir_exec_stmt_cjmp_def,CaseEq"option",bir_programTheory.bir_exec_stmt_jmp_def,bir_programTheory.bir_state_set_typeerror_def,bir_programTheory.bir_exec_stmt_jmp_to_label_def,pairTheory.ELIM_UNCURRY,stmt_generic_step_def,bir_programTheory.bir_state_is_terminated_def,bir_programTheory.bir_exec_stmtB_def,bir_get_stmt_generic]
+      >> gvs[bir_programTheory.bir_exec_stmt_assert_def,bir_programTheory.bir_exec_stmt_assume_def,CaseEq"option",bir_programTheory.bir_state_set_typeerror_def,bir_programTheory.bir_exec_stmt_observe_def]
+      >> BasicProvers.every_case_tac
+      >> gvs[]
+    )
+    >> qmatch_assum_rename_tac `bir_get_stmt p _ = BirStmt_Generic $ BStmtE e`
+    >> Cases_on `e`
+    >> fs[bir_programTheory.bir_exec_stmtE_def,bir_programTheory.bir_exec_stmt_jmp_def,bir_programTheory.bir_exec_stmt_jmp_to_label_def,bir_programTheory.bir_exec_stmt_cjmp_def,bir_programTheory.bir_exec_stmt_halt_def]
+    >> BasicProvers.every_case_tac
+    >> gvs[bir_programTheory.bir_exec_stmt_assert_def,bir_programTheory.bir_exec_stmt_assume_def,CaseEq"option",bir_programTheory.bir_state_set_typeerror_def,bir_programTheory.bir_exec_stmt_observe_def]
+  )
+QED
+
+(* a positive fwdb at some location  l  comes from an earlier successful store
+ * to this location *)
+
+Theorem pos_fwdb_is_fulfil:
+  !tr i cid p st st' t l.
+  wf_trace tr /\ i < LENGTH tr
+  /\ progressing_trace tr
+  /\ FLOOKUP (FST $ HD tr) cid = SOME $ Core cid p st'
+  /\ st'.bst_fwdb l = <|fwdb_time := 0; fwdb_view := 0; fwdb_xcl := F|>
+  /\ FLOOKUP (FST $ EL i tr) cid = SOME $ Core cid p st
+  /\ 0 < (st.bst_fwdb l).fwdb_time
+  ==>
+    ?j t st st'. j < i
+    /\ is_fulfil cid t (EL j tr) (FST $ EL (SUC j) tr)
+    /\ FLOOKUP (FST $ EL j tr) cid = SOME $ Core cid p st
+    /\ FLOOKUP (FST $ EL (SUC j) tr) cid = SOME $ Core cid p st'
+    /\ l = (EL (PRE t) $ SND $ EL j tr).loc
+    /\ cid = (EL (PRE t) $ SND $ EL j tr).cid
+    /\ st.bst_fwdb l <> st'.bst_fwdb l
+    /\ same_state_prop_range cid tr (SUC j) i (λst. st.bst_fwdb l)
+Proof
+  rpt strip_tac
+  >> qabbrev_tac `P = λj. ?k. k = i - j /\ 0 < j /\ j < i
+    /\ is_fulfil cid t (EL k tr) (FST $ EL (SUC k) tr)
+    /\ FLOOKUP (FST $ EL k tr) cid = SOME $ Core cid p st
+    /\ FLOOKUP (FST $ EL (SUC k) tr) cid = SOME $ Core cid p st'
+    /\ l = (EL (PRE t) $ SND $ EL k tr).loc
+    /\ cid = (EL (PRE t) $ SND $ EL k tr).cid
+    /\ st.bst_fwdb l <> st'.bst_fwdb l`
+  >> reverse $ Cases_on `?i. P i`
+  >- (
+    fs[Abbr`P`,DISJ_EQ_IMP,AND_IMP_INTRO]
+    >> `same_state_prop cid (FST $ HD tr) (FST $ EL i tr) (λst. st.bst_fwdb l)` by (
+      cheat
+    )
+    >> gs[same_state_prop_def]
+  )
+  >> dxrule_then assume_tac arithmeticTheory.WOP
+  >> gs[Abbr`P`,DISJ_EQ_IMP,AND_IMP_INTRO]
+  >> qhdtm_assum `is_fulfil` $ irule_at Any
+  >> fs[]
+(* using
+is_fulfil_xcl_bst_fwdb_eq
+*)
+  >> cheat
+QED
+
+Theorem is_read_xcl_timestamp_less_or_bst_xclb:
+  !tr i j cid p st st' t.
+  wf_trace tr /\ SUC i < LENGTH tr
+  /\ progressing_trace tr
+  /\ core_runs_spinlock cid $ FST $ HD tr
+  /\ is_read_xcl cid t (EL i tr) (FST $ EL (SUC i) tr)
+  /\ FLOOKUP (FST $ EL i tr) cid = SOME $ Core cid p st
+  /\ FLOOKUP (FST $ EL (SUC i) tr) cid = SOME $ Core cid p st'
+  ==> IS_SOME st'.bst_xclb /\ t <= (THE st'.bst_xclb).xclb_view
+Proof
+  rpt gen_tac >> strip_tac
+  >> drule_at_then (Pat `is_read_xcl _ _ _ _`) assume_tac is_read_xcl_parstep_nice_eq
+  >> Cases_on `0 < t`
+  >> gvs[FLOOKUP_UPDATE,mem_read_view_def,mem_read_def]
+  >> qmatch_asmsub_abbrev_tac `mem_read MM ll tt`
+  >> qspecl_then [`tt`,`MM`,`ll`] assume_tac mem_read_EL_SND_loc
+  >> gvs[optionTheory.IS_SOME_EXISTS,is_read_xcl_def]
+  >> rpt disj2_tac
+  >> IF_CASES_TAC
+  >> fs[FLOOKUP_UPDATE]
+  >> qhdtm_x_assum `is_certified` kall_tac
+  >> qmatch_asmsub_abbrev_tac `_.bst_fwdb l`
+  >> drule_then (drule_then $ qspec_then `0` assume_tac) wf_trace_cid_backward
+  >> drule_at (Pat `FLOOKUP (FST $ EL i tr) _ = _`) pos_fwdb_is_fulfil
+  >> gs[]
+  >> disch_then $ qspec_then `l` mp_tac
+  >> impl_tac
+  >- fs[core_runs_spinlock_def,core_runs_prog_def,bir_programTheory.bir_state_init_def]
+  (* there is no earlier store to location l in this thread *)
+  (* the address location of the spinlock_var is never changed *)
+  >> cheat
+QED
+
+(* a core in the critical section has run an earlier exclusive lr-sc pair *)
+
+Theorem in_crit_lr_sc:
+  !tr i cid p st st'.
+  wf_trace tr /\ i < LENGTH tr
+  /\ progressing_trace tr
+  /\ core_runs_spinlock cid $ FST $ HD tr
+  /\ FLOOKUP (FST (EL i tr)) cid = SOME (Core cid p st)
+  /\ in_crit (Core cid p st)
+  ==> ?t1 i1 t2 i2. lr_sc cid tr t1 i1 t2 i2 /\ i2 < i
+Proof
+  rpt strip_tac
+  >> drule_all_then strip_assume_tac in_crit_is_fulfil_xcl
+  >> fs[lr_sc_def]
+  >> qhdtm_assum `is_fulfil_xcl` $ irule_at Any
+  >> drule_all_then strip_assume_tac wf_trace_cid_backward'
+  >> drule_at_then (Pat `is_fulfil_xcl _ _ _ _`) assume_tac is_fulfil_xcl_is_read_xcl
+  >> imp_res_tac is_fulfil_xcl_is_fulfil
+  >> drule_at_then (Pat `is_fulfil _ _ _ _`) assume_tac is_fulfil_to_memory
+  >> gs[]
+  >> qhdtm_assum `is_read_xcl` $ irule_at Any
+  >> fs[]
+  >> conj_asm1_tac
+  >- (
+    drule_at_then (Pat `is_fulfil_xcl _ _ _ _`) assume_tac is_fulfil_xcl_bst_xclb_less_timestamp
+    >> drule_at (Pat `FLOOKUP _ _ = _`) wf_trace_cid_backward
+    >> qmatch_assum_rename_tac `j' < j`
+    >> disch_then (fn thm =>
+      qspec_then `j'` assume_tac thm
+      >> qspec_then `SUC j'` assume_tac thm)
+    >> drule_at_then (Pat `is_read_xcl _ _ _ _`) assume_tac is_read_xcl_timestamp_less_or_bst_xclb
+    >> gs[]
+    >> first_x_assum $ drule_at_then Any assume_tac
+    >> gs[]
+  )
+  >> conj_tac
+  >- (
+    fs[same_state_prop_range_def]
+    (* by induction *)
+    >> cheat
+  )
+  (* a property of the spinlock program *)
+  >> cheat
+QED
+
+(* a successful lr-sc takes the lock *)
+(* For a full spinlock program the lr is necessary to distinguish sc from any
+ * other later write *)
+
+Theorem lr_sc_takes_lock:
+  !cid tr t1 i1 t2 i2 p st.
+  wf_trace tr /\ progressing_trace tr
+  /\ core_runs_spinlock cid $ FST $ HD tr
+  /\ lr_sc cid tr t1 i1 t2 i2
+  /\ FLOOKUP (FST $ EL i2 tr) cid = SOME $ Core cid p st
+  ==> ?loc st'.
+    oEL (PRE t2) (SND $ EL (SUC i2) tr)
+      = SOME <| cid := cid; loc := loc; val := lock_taken |>
+    /\ bir_eval_view_of_exp (BExp_Den spinlock_var) st.bst_viewenv < t2
+    /\ bir_eval_exp (BExp_Den spinlock_var) st.bst_environ = SOME loc
+    /\ bir_eval_view_of_exp
+        (BExp_Cast BIExp_LowCast (BExp_Const $ Imm64 0w) Bit32)
+        st.bst_viewenv < t2
+    /\ FLOOKUP (FST $ EL (SUC i2) tr) cid = SOME $ Core cid p st'
+    /\ bir_env_update "x6" (BVal_Imm (Imm64 0w)) (BType_Imm Bit64) st.bst_environ
+      = SOME st'.bst_environ
+Proof
+  rpt gen_tac >> strip_tac
+  >> fs[lr_sc_def]
+  >> imp_res_tac is_fulfil_xcl_is_fulfil
+  >> fs[is_fulfil_xcl_def]
+  >> drule_all_then assume_tac wf_trace_core_runs_spinlock_FLOOKUP
+  >> dxrule_at_then (Pat `is_fulfil _ _ _ _`) assume_tac is_fulfil_parstep_nice_eq
+  >> gvs[FLOOKUP_UPDATE,bir_get_stmt_bir_spinlock_prog_BirStmt_Write_EQ,bst_pc_tuple_def,bir_programTheory.bir_pc_next_def,oEL_THM,bir_eval_exp_view_def]
+  >> conj_asm1_tac
+  >- (
+    qmatch_rename_tac `v = lock_taken`
+    >> qpat_x_assum `SOME v = bir_eval_exp _ _` mp_tac
+    >> EVAL_TAC
+  )
+  >> EVAL_TAC
+  >> simp[bir_spinlock_prog_def,fulfil_update_env_def,bir_programTheory.bir_programcounter_t_component_equality,AllCaseEqs(),bir_envTheory.bir_var_name_def,bir_envTheory.bir_var_type_def]
+QED
+
+(* a successful lr-sc must have read a free lock *)
+
+Theorem lr_sc_fails:
+  !cid tr t1 i1 t2 i2 p st loc.
+  wf_trace tr /\ progressing_trace tr
+  /\ core_runs_spinlock cid $ FST $ HD tr
+  /\ lr_sc cid tr t1 i1 t2 i2
+  /\ FLOOKUP (FST $ EL i1 tr) cid = SOME $ Core cid p st
+  /\ bir_eval_exp (BExp_Den spinlock_var) st.bst_environ = SOME loc
+  ==> 0 < t1 /\ mem_read (SND $ EL (SUC i1) tr) loc t1 = SOME lock_free
+Proof
+  rpt gen_tac >> strip_tac
+  >> conj_asm1_tac
+  >- (
+    cheat (* initially a lock is not taken *)
+  )
+  >> drule_at_then (Pat `FLOOKUP _ _ = _`) assume_tac wf_trace_core_runs_spinlock_FLOOKUP
+  >> `?st' new_env v.
+     mem_read (SND (EL i1 tr)) loc t1 = SOME v
+     /\ FLOOKUP (FST $ EL (SUC i1) tr) cid = SOME $ Core cid p st'
+     /\ env_update_cast64 (bir_var_name (BVar "x5" (BType_Imm Bit64))) v
+          (bir_var_type (BVar "x5" (BType_Imm Bit64))) st.bst_environ
+          = SOME st'.bst_environ
+    /\ bst_pc_tuple st'.bst_pc = (BL_Address $ Imm64 12w, 3)` by (
+    fs[lr_sc_def]
+    >> drule_at_then (Pat `is_read_xcl _ _ _ _`) assume_tac is_read_xcl_parstep_nice_eq
+    >> gvs[is_read_xcl_def,FLOOKUP_UPDATE,bir_get_stmt_bir_spinlock_prog_BirStmt_Read_EQ,bir_programTheory.bir_pc_next_def,oEL_THM,bir_eval_exp_view_def,bst_pc_tuple_def]
+  )
+  >> cheat
+  (*
+lr_sc_takes_lock
+
+m`sl_step _ _`
+
+       a0 = (BL_Address (Imm64 12w),3) ∧ a1 = (BL_Address (Imm64 16w),0) ∨
+       a0 = (BL_Address (Imm64 16w),0) ∧ a1 = (BL_Address (Imm64 12w),0) ∨
+       a0 = (BL_Address (Imm64 16w),0) ∧ a1 = (BL_Address (Imm64 20w),0) ∨
+       a0 = (BL_Address (Imm64 20w),0) ∧ a1 = (BL_Address (Imm64 20w),1) ∨
+       a0 = (BL_Address (Imm64 20w),1) ∧ a1 = (BL_Address (Imm64 20w),2) ∨
+       a0 = (BL_Address (Imm64 20w),2) ∧ a1 = (BL_Address (Imm64 20w),5) ∨
+
+  >> fs[mem_read_thm,mem_read_aux_def,oEL_THM]
+  *)
+QED
+
+(* lock already taken *)
+
+Theorem lr_sc_pair_locked:
+  !tr cid cid' t1 t2 i1 i2 t1' t2' j1 j2.
+  wf_trace tr /\ progressing_trace tr
+  /\ core_runs_spinlock cid $ FST $ HD tr
+  /\ core_runs_spinlock cid' $ FST $ HD tr
+  /\ lr_sc cid tr t1 i1 t2 i2
+  /\ lr_sc cid' tr t1' j1 t2' j2
+  /\ t2 <= t1'
+  /\ (EL (PRE t1') $ SND $ EL (SUC i2) tr).loc = XX spinlock_var
+  /\ (EL (PRE t1') $ SND $ EL (SUC i2) tr).val = lock_taken
+  /\ cid <> cid'
+  /\ (EL (PRE t2) $ SND $ EL (SUC i2) tr).loc
+    = (EL (PRE t2') $ SND $ EL (SUC j2) tr).loc
+  ==> F
+Proof
+  cheat
+(*
+cid' reads at t1' that the lock is taken,
+thus the fulfil transition j2 -> SUC j2 is not possible
+*)
+QED
+
+(* wlog we have the last lr before the store *)
+
+Theorem lr_sc_without_interleaving_read:
+  !tr cid cid' t1 t2 i1 i2 t1' t2' j1 j2.
+  wf_trace tr /\ progressing_trace tr
+  /\ lr_sc cid tr t1 i1 t2 i2
+  ==> ?t1' i1'. lr_sc cid tr t1' i1' t2 i2
+    /\ t1 <= t1' /\ i1 <= i1'
+    /\ !i. i1 <= i /\ i < i1'
+      ==> ~is_read_xcl cid t1' (EL i1' tr) (FST $ EL (SUC i1') tr)
+Proof
+  cheat
+QED
+
+Theorem init_unique:
+  !i tr. wf_trace tr /\ wf_trace1 tr
+  /\ progressing_trace tr
+  /\ SUC i < LENGTH tr
+  /\ cores_run_spinlock $ FST $ HD tr
+  /\ invariant (FST $ EL i tr)
+  ==> invariant (FST $ EL (SUC i) tr)
+Proof
+  rw[invariant_def]
+  >> imp_res_tac cores_run_spinlock_init
+  >> drule_all_then strip_assume_tac wf_trace_parstep_EL
+  >> imp_res_tac parstep_nice_EX_FLOOKUP
+  >> drule_all_then strip_assume_tac parstep_nice_FLOOKUP
+  >> drule_all_then assume_tac wf_trace_core_runs_spinlock_FLOOKUP'
+  >> Cases_on `st.bst_pc = st'.bst_pc`
+  >- (
+    fs[unique_def,in_crit_def,parstep_nice_def,parstep_cases]
+    >> rw[FLOOKUP_UPDATE,DISJ_EQ_IMP]
+    >> spose_not_then assume_tac
+    >> gvs[FLOOKUP_UPDATE]
+    >> first_x_assum $ dxrule_at $ Pat `FLOOKUP _ _ = _`
+    >> disch_then $ dxrule_at $ Pat `FLOOKUP _ _ = _`
+    >> fs[in_crit_def]
+  )
+  >> rev_drule_all_then assume_tac reachable_pc_sl_step
+  >> reverse $ Cases_on `in_crit $ THE $ FLOOKUP (FST $ EL (SUC i) tr) cid`
+  >- (
+    Q.ISPEC_THEN `in_crit` rev_drule FLOOKUP_NOT_unique_eq
+    >> disch_then $ drule_at Any
+    >> gvs[optionTheory.option_CLAUSES,parstep_nice_def,parstep_cases,FLOOKUP_UPDATE]
+    >> disch_then irule
+    >> drule_then (drule_at Any) in_crit_sl_step
+    >> fs[]
+  )
+  >> gvs[sl_step_cases,bst_pc_tuple_def,in_crit_def,bir_programTheory.bir_programcounter_t_component_equality]
+  >> reverse $ Cases_on `
+    ?cid p st. FLOOKUP (FST $ EL i tr) cid = SOME $ Core cid p st
+    /\ in_crit $ Core cid p st
+    `
+  >- (
+    rw[unique_def,FLOOKUP_UPDATE]
+    >> spose_not_then assume_tac
+    >> fs[DISJ_EQ_IMP]
+    >> qmatch_assum_rename_tac `FLOOKUP _ id' = SOME $ xx` >> Cases_on `xx`
+    >> qmatch_assum_rename_tac `FLOOKUP _ id = SOME $ xx` >> Cases_on `xx`
+    >> drule_then imp_res_tac wf_trace1_FLOOKUP
+    >> gvs[]
+    >> drule_at Any wf_trace_cid_backward1
+    >> qpat_x_assum `FLOOKUP _ _ = SOME _` mp_tac
+    >> drule_at Any wf_trace_cid_backward1
+    >> rpt strip_tac
+    >> gvs[]
+    >> PRED_ASSUM is_forall imp_res_tac
+    >> `id <> cid /\ id' <> cid` by (
+      conj_tac
+      >> spose_not_then assume_tac
+      >> gvs[]
+      >> rev_dxrule_at (Pat $ `FLOOKUP _ _ = _`) wf_trace_unchanged
+      >> disch_then $ dxrule_at_then (Pat `FLOOKUP _ _ = _`) assume_tac
+      >> gvs[]
+      >> gs[bir_programTheory.bir_state_t_component_equality,bir_programTheory.bir_programcounter_t_component_equality,in_crit_def]
+    )
+    >> Cases_on `parstep_nice id (EL i tr) (EL (SUC i) tr)`
+    >- imp_res_tac progressing_trace_cid_eq
+    >> Cases_on `parstep_nice id' (EL i tr) (EL (SUC i) tr)`
+    >- imp_res_tac progressing_trace_cid_eq
+    >> ntac 2 $ dxrule_at (Pat `~parstep_nice _ _ _`) wf_trace_NOT_parstep_nice_state_EQ'
+    >> rpt strip_tac
+    >> rfs[]
+    >> gvs[]
+  )
+  >> fs[]
+  >> `cid <> cid'` by (
+    spose_not_then assume_tac
+    >> gvs[in_crit_def]
+  )
+  >> drule_all_then assume_tac progressing_trace_state'
+  >> spose_not_then kall_tac
+  >> `core_runs_spinlock cid (FST $ HD tr)
+    /\ core_runs_spinlock cid' (FST $ HD tr)` by (
+    drule_at (Pat `FLOOKUP _ _ = _`) wf_trace_cid_backward'
+    >> disch_then $ qspec_then `0` assume_tac
+    >> gs[cores_run_spinlock_def]
+  )
+  >> `in_crit $ Core cid p st'` by fs[in_crit_def,bst_pc_tuple_def,bir_programTheory.bir_programcounter_t_component_equality]
+  >> ntac 2 $ dxrule_at_then (Pat`core_runs_spinlock cid _`) (qspec_then `SUC i` assume_tac) in_crit_lr_sc
+  >> gs[]
+  >> qmatch_assum_rename_tac `lr_sc cid tr t1 i1 t2 i2`
+  >> qmatch_assum_rename_tac `lr_sc cid' tr t1' i1' t2' i2'`
+(*
+assume there is interleaving read lr-lr-..-sc
+lr_sc_without_interleaving_read
+*)
+  >> Cases_on `t1 < t1' /\ t1' < t2`
+  >- (
+    fs[]
+    >> dxrule_at (Pat `lr_sc _ _ _ _ _ _`) lr_sc_interleaved_pair
+    >> rpt $ disch_then $ drule
+    >> fs[]
+    >> cheat (* lookup location of writes from spinlock program *)
+  )
+  >> Cases_on `t1 < t2' /\ t2' < t2`
+  >- (
+    >> dxrule_at (Pat `lr_sc _ _ _ _ _ _`) lr_sc_interleaved_pair'
+    >> rpt $ disch_then $ drule
+    >> fs[]
+    >> cheat (* lookup location of writes from spinlock program *)
+  )
+  >> Cases_on `t1 = t1'`
+  >- (
+    cheat (* impossible by program flow *)
+  )
+  >> Cases_on `t2 = t2'`
+  >- (
+    cheat (* impossible as cid is tied to *)
+  )
+  >> Cases_on `t1 = t2'`
+  >- cheat
+  >> cheat (* lr_sc_pair_locked *)
+QED
+
+val _ = export_theory();
