examples/spinlock/spinlockRefinementScript.sml
@@ -1,0 +1,109 @@
+
+open HolKernel Parse boolLib bossLib;
+open rich_listTheory listTheory arithmeticTheory finite_mapTheory ;
+open bir_lifter_interfaceLib ;
+(* bir_promisingTheory ; *)
+open bir_promisingGhostTheory;
+open tracesTheory tracestepTheory spinlockTheory ;
+
+val _ = new_theory "spinlockRefinement";
+
+val _ = set_trace "bir_inst_lifting.DEBUG_LEVEL" 2;
+
+val (bir_spinlockfull_progbin_def, bir_spinlockfull_prog_def, bir_is_lifted_prog_spinlockfull) = lift_da_and_store_mc_riscv
+          "spinlockfull"
+          "spinlockfull.da"
+          ((Arbnum.fromInt 0), (Arbnum.fromInt 0x1000000));
+
+(*
+returns the word with the cid's bit set to 1
+0...010...0
+     ^
+    cid
+*)
+(* TODO functions between num and word, n2w? *)
+
+Definition cid2w_def:
+  cid2w (cid : num) = BExp_Const $ Imm64 (ARB : word64)
+End
+
+(*
+
+- need assumption that GHOST.crit contains only zeros (= free)
+
+check "ghost only" expression evaluations
+- all memory assignment sub-expressions need to be ghost memories
+- only assignment to ghost
+
+*)
+
+(* A spinlock definition that is parametrised by its core id.
+ * The core id is used marking the lock taken. *)
+
+Definition bir_spinlock_def:
+  bir_spinlock cid =
+  BirProgram [
+  (* lock block *)
+  <|bb_label := BL_Address_HC (Imm64 0w) "";
+    bb_mc_tags := SOME <|mc_atomic := T; mc_acq := F; mc_rel := F|>;
+    bb_statements :=
+      [
+        (* _tmp := _GHOST.crit *)
+        BStmt_Assign (BVar "_tmp" $ BType_Imm Bit64)
+          (* BExp_Load mem_e a_e endianness type *)
+            $ BExp_Load (BExp_Den $ BVar "_GHOST" $ BType_Mem Bit64 Bit8)
+                      (BExp_Den $ BVar "crit" $ BType_Imm Bit64)
+                      BEnd_LittleEndian Bit32;
+        (* _is_locked := (_tmp != 0) *)
+        BStmt_Assign (BVar "_is_locked" $ BType_Imm Bit64)
+          $ BExp_IfThenElse
+              (BExp_BinExp BIExp_And
+                (BExp_Const $ Imm64 0w)
+                (BExp_Den $ BVar "_tmp" $ BType_Imm Bit64))
+              (BExp_Const $ Imm64 1w)
+              (BExp_Const $ Imm64 0w);
+        (* lock if possible *)
+        BStmt_Assign (BVar "_ignore" $ BType_Imm Bit64)
+          $ BExp_Store (BExp_Den $ BVar "_GHOST" $ BType_Mem Bit64 Bit8)
+            (BExp_Den $ BVar "crit" $ BType_Imm Bit64)
+            BEnd_LittleEndian
+            $ BExp_IfThenElse
+                (BExp_Den $ BVar "_is_locked" $ BType_Imm Bit64)
+                (BExp_Den $ BVar "_tmp" $ BType_Imm Bit64)
+                (cid2w cid);
+      ];
+    (* spin on _is_locked *)
+    bb_last_statement := 
+        BStmt_CJmp
+          (BExp_Den $ BVar "_is_locked" $ BType_Imm Bit64)
+          (BLE_Label $ BL_Address $ Imm64 0w)
+          (BLE_Label $ BL_Address $ Imm64 4w);
+  |>;
+  (* unlock *)
+  <|bb_label := BL_Address_HC (Imm64 4w) "";
+    bb_mc_tags := SOME <|mc_atomic := F; mc_acq := F; mc_rel := F|>;
+    bb_statements :=
+      [
+(*
+reset lock availability for cid by writing
+_GHOST.crit := (1...101...1   AND   _GHOST.crit)
+                     ^
+                    cid
+*)
+      BStmt_Assign
+        (BVar "_GHOST" $ BType_Mem Bit64 Bit8)
+        $ BExp_Store (BExp_Den $ BVar "_GHOST" $ BType_Mem Bit64 Bit8)
+          (BExp_Den $ BVar "crit" $ BType_Imm Bit64)
+          BEnd_LittleEndian
+          $ BExp_BinExp BIExp_And
+              (BExp_Load (BExp_Den $ BVar "_GHOST" $ BType_Mem Bit64 Bit8)
+                (BExp_Den $ BVar "crit" $ BType_Imm Bit64)
+                BEnd_LittleEndian Bit32)
+              $ BExp_UnaryExp BIExp_Not $ cid2w cid;
+      ];
+    bb_last_statement := BStmt_Jmp $ BLE_Label $ BL_Address $ Imm64 8w
+  |>
+  ] : string bir_program_t
+End
+
+val _ = export_theory();
