examples/spinlock/tracestepScript.sml
@@ -1,0 +1,1727 @@
+open HolKernel Parse boolLib bossLib;
+
+open bir_lifter_interfaceLib;
+
+val _ = new_theory "tracestep";
+
+open bir_promisingTheory rich_listTheory listTheory arithmeticTheory tracesTheory;
+open finite_mapTheory;
+
+Theorem IS_PREFIX_EL:
+  !l2 l1 n. IS_PREFIX l2 l1 /\ n < LENGTH l1
+  ==> EL n l1 = EL n l2
+Proof
+  fs[IS_PREFIX_APPEND,EL_APPEND1,PULL_EXISTS]
+QED
+
+Theorem LT3 =
+  (REWRITE_CONV [GSYM rich_listTheory.COUNT_LIST_COUNT,
+    GSYM pred_setTheory.IN_COUNT]
+    THENC EVAL) ``n < 3n``
+
+Theorem LT5 =
+  (REWRITE_CONV [GSYM rich_listTheory.COUNT_LIST_COUNT,
+    GSYM pred_setTheory.IN_COUNT]
+    THENC EVAL) ``n < 5n``
+
+Theorem mem_read_thm:
+  !t l M. 0 < t
+  ==> mem_read M l t = mem_read_aux l (oEL (PRE t) M)
+Proof
+  Cases >> fs[mem_read_def]
+QED
+
+(*
+ * equality of projection of states
+ *)
+
+Definition same_state_prop_def:
+  same_state_prop cid st1 st2 f =
+    !p st st'.
+      FLOOKUP st1 cid = SOME $ Core cid p st
+      /\ FLOOKUP st2 cid = SOME $ Core cid p st'
+      ==> f st = f st'
+End
+
+Definition same_state_prop_range_def:
+  same_state_prop_range cid tr i j f <=>
+    i <= j /\ !k. i <= k /\ k < j
+      ==> same_state_prop cid (FST $ EL k tr) (FST $ EL (SUC k) tr) f
+End
+
+Theorem same_state_prop_range_simp[simp]:
+  same_state_prop_range cid tr i i f
+Proof
+  fs[same_state_prop_range_def]
+QED
+
+Theorem same_state_prop_range_add:
+  same_state_prop_range cid tr i j f
+  /\ same_state_prop_range cid tr j k f
+  ==> same_state_prop_range cid tr i k f
+Proof
+  rw[same_state_prop_range_def]
+  >> qmatch_assum_rename_tac `kk < k`
+  >> Cases_on `j <= kk`
+  >- (first_x_assum irule >> fs[])
+  >> fs[NOT_LESS_EQUAL]
+QED
+
+Theorem same_state_prop_range_SUC:
+  same_state_prop_range cid tr i (SUC j) f
+  /\ i <= j
+  ==> same_state_prop_range cid tr i j f
+Proof
+  rw[same_state_prop_range_def]
+QED
+
+Theorem same_state_prop_range_prop:
+  wf_trace tr /\ SUC k < LENGTH tr
+  /\ same_state_prop_range cid tr i (SUC k) f
+  /\ same_state_prop cid (FST (EL i tr)) (FST $ EL k tr) f
+  ==> same_state_prop cid (FST (EL i tr)) (FST (EL (SUC k) tr)) f
+Proof
+  rw[same_state_prop_def,same_state_prop_range_def]
+  >> drule_at_then (Pat `FLOOKUP _ _ = _`) assume_tac wf_trace_cid_backward1
+  >> dxrule_then strip_assume_tac $ iffLR LESS_OR_EQ
+  >> gvs[PULL_FORALL,AND_IMP_INTRO]
+  >> first_x_assum $ drule_at $ Pat `FLOOKUP _ _ = _`
+  >> fs[]
+QED
+
+Theorem same_state_prop_indexes:
+  !i j cid tr f.
+  wf_trace tr /\ j < LENGTH tr
+  /\ same_state_prop_range cid tr i j f
+  ==> same_state_prop cid (FST $ EL i tr) (FST $ EL j tr) f
+Proof
+  rpt gen_tac
+  >> Induct_on `j - i`
+  >> rpt strip_tac
+  >- (
+    fs[same_state_prop_range_def,relationTheory.reflexive_def]
+    >> dxrule_all_then assume_tac $ iffLR $ GSYM arithmeticTheory.EQ_LESS_EQ
+    >> rw[same_state_prop_def]
+    >> gs[]
+  )
+  >> gvs[AND_IMP_INTRO,Once SUB_LEFT_EQ]
+  >> first_x_assum $ qspecl_then [`i+v`,`i`] mp_tac
+  >> impl_tac
+  >- (
+    fs[]
+    >> irule same_state_prop_range_SUC
+    >> fs[ADD1]
+  )
+  >> strip_tac
+  >> drule_at (Pat `same_state_prop _ _ _ _`) same_state_prop_range_prop
+  >> fs[ADD1]
+QED
+
+Theorem wf_trace_NOT_parstep_nice_same_state_prop:
+  wf_trace tr
+  /\ SUC i < LENGTH tr
+  /\ progressing_trace tr
+  /\ FLOOKUP (FST (EL i tr)) cid = SOME (Core cid p st)
+  /\ ~parstep_nice cid (EL i tr) (EL (SUC i) tr)
+  ==> same_state_prop cid (FST $ EL i tr) (FST $ EL (SUC i) tr) I
+Proof
+  rpt strip_tac
+  >> drule_all_then strip_assume_tac wf_trace_cid_forward1
+  >> drule_at (Pat `~parstep_nice _ _ _`) wf_trace_NOT_parstep_nice_state_EQ'
+  >> fs[same_state_prop_def]
+QED
+
+(* general utility to get the previous state that satisfies a property ~P *)
+
+Definition prev_state_P_def:
+  prev_state_P tr i k cid P <=>
+     i <= k
+     /\ k < LENGTH tr
+     /\ IS_SOME $ FLOOKUP (FST (EL i tr)) cid
+     /\ (!j. i <= j /\ j < k /\ parstep_nice cid (EL j tr) (EL (SUC j) tr) ==>
+         P cid tr j (SUC j))
+     ==> P cid tr i k
+End
+
+(*
+  ∀j. SUC k ≤ j ∧ j < i ∧ parstep_nice cid (EL j tr) (EL (SUC j) tr) ⇒
+      P cid tr j (SUC j)
+*)
+
+Theorem previous_state_change_P:
+  !P i cid tr p st.
+  wf_trace tr /\ i < LENGTH tr
+  /\ progressing_trace tr
+  /\ FLOOKUP (FST (EL i tr)) cid = SOME $ Core cid p st
+  /\ (!l i. prev_state_P tr l i cid P)
+  ==>
+    P cid tr 0 i
+    \/ ?j. j < i
+      /\ parstep_nice cid (EL j tr) (EL (SUC j) tr)
+      /\ ~P cid tr j (SUC j)
+      /\ P cid tr (SUC j) i
+Proof
+  rpt strip_tac
+  >> qabbrev_tac `Q = λj. LENGTH tr - j < i
+    /\ LENGTH tr - j < LENGTH tr /\ 0 <= LENGTH tr - j
+    /\ parstep_nice cid (EL (LENGTH tr - j) tr) (EL (SUC $ LENGTH tr - j) tr)
+    /\ ~P cid tr (LENGTH tr - j) (SUC $ LENGTH tr - j)
+  `
+  >> reverse $ Cases_on `?i. Q i`
+  >- (
+    disj1_tac
+    >> unabbrev_all_tac
+    >> pop_assum mp_tac
+    >> REWRITE_TAC[NOT_EXISTS_THM]
+    >> CONV_TAC $ DEPTH_CONV BETA_CONV
+    >> REWRITE_TAC[DISJ_EQ_IMP,AND_IMP_INTRO,DE_MORGAN_THM]
+    >> qho_match_abbrev_tac `(!x. A i x) ==> _`
+    >> disch_then assume_tac
+    >> `(!x. A i x) <=> !j. j < i
+      /\ parstep_nice cid (EL j tr) (EL (SUC j) tr) ==> P cid tr j (SUC j)` by (
+      rw[EQ_IMP_THM,Abbr`A`]
+      >> first_x_assum $ qspec_then `LENGTH tr - j` mp_tac
+      >> fs[]
+    )
+    >> qpat_x_assum `Abbrev _` kall_tac
+    >> fs[prev_state_P_def]
+    >> first_x_assum irule
+    >> drule_at_then (Pat `FLOOKUP _ _ = _`) (qspec_then `0` assume_tac) wf_trace_cid_backward
+    >> gs[optionTheory.IS_SOME_EXISTS]
+  )
+  >> dxrule_then assume_tac arithmeticTheory.WOP
+  >> disj2_tac
+  >> unabbrev_all_tac
+  >> pop_assum mp_tac
+  >> REWRITE_TAC[NOT_EXISTS_THM]
+  >> CONV_TAC $ DEPTH_CONV BETA_CONV
+  >> REWRITE_TAC[DISJ_EQ_IMP,AND_IMP_INTRO,DE_MORGAN_THM]
+  >> qho_match_abbrev_tac `(?x. _ x /\ !m. B x m) ==> _`
+  >> disch_then strip_assume_tac
+  >> qpat_x_assum `_ x` mp_tac
+  >> CONV_TAC $ DEPTH_CONV BETA_CONV
+  >> disch_then strip_assume_tac
+  >> qmatch_assum_abbrev_tac `parstep_nice cid (EL k tr) _`
+  >> qhdtm_x_assum `parstep_nice` $ irule_at Any
+  >> asm_rewrite_tac[]
+  >> qpat_x_assum `!a b. prev_state_P _ a b _ _` $ irule o REWRITE_RULE[prev_state_P_def]
+  >> simp[]
+  >> conj_tac
+  >- (
+    PRED_ASSUM is_forall $ qspec_then `LENGTH tr - l` $ (qspec_then `tr` mp_tac) o GEN_ALL
+    >> unabbrev_all_tac
+    >> fs[]
+  )
+  >> drule_at_then (Pat `FLOOKUP _ _ = _`) (qspec_then `SUC k` assume_tac) wf_trace_cid_backward
+  >> gs[optionTheory.IS_SOME_EXISTS]
+QED
+
+(* for a core in a trace either there is previous progress,
+ * or the core has never progressed *)
+
+Theorem previous_state_change:
+  !i cid tr p st.
+  wf_trace tr /\ i < LENGTH tr
+  /\ progressing_trace tr
+  /\ FLOOKUP (FST (EL i tr)) cid = SOME $ Core cid p st
+  ==>
+    same_state_prop_range cid tr 0 i I
+    \/ ?j. j < i
+      /\ parstep_nice cid (EL j tr) (EL (SUC j) tr)
+      /\ same_state_prop_range cid tr (SUC j) i I
+Proof
+  rpt strip_tac
+  >> drule previous_state_change_P
+  >> rpt $ disch_then $ drule_at Any
+  >> disch_then $ qspec_then `λcid tr i j. same_state_prop_range cid tr i j I` mp_tac
+  >> impl_tac
+  >- (
+    rw[prev_state_P_def,same_state_prop_range_def,same_state_prop_def]
+    >> first_x_assum drule
+    >> dsimp[same_state_prop_range_def,LESS_OR_EQ,same_state_prop_def]
+    >> qmatch_goalsub_abbrev_tac `(A ==> _) ==> _`
+    >> Cases_on `A`
+    >> fs[]
+    >> drule_at (Pat `~parstep_nice _ _ _`) wf_trace_NOT_parstep_nice_state_EQ'
+    >> fs[]
+  )
+  >> rw[]
+  >> fs[]
+  >> disj2_tac
+  >> goal_assum $ drule_at Any
+  >> fs[]
+QED
+
+(*
+Old proof
+
+Theorem previous_state_change:
+  !i cid tr p st.
+  wf_trace tr /\ i < LENGTH tr
+  /\ progressing_trace tr
+  /\ FLOOKUP (FST (EL i tr)) cid = SOME $ Core cid p st
+  ==>
+    same_state_prop_range cid tr 0 i I
+    \/ ?j. j < i
+      /\ parstep_nice cid (EL j tr) (EL (SUC j) tr)
+      /\ same_state_prop_range cid tr (SUC j) i I
+Proof
+  rpt strip_tac
+  >> qabbrev_tac `P = λj. LENGTH tr - j < i /\ 1 < j /\ j <= LENGTH tr
+    /\ parstep_nice cid (EL (LENGTH tr - j) tr) (EL (SUC $ LENGTH tr - j) tr)`
+  >> reverse $ Cases_on `?i. P i`
+  >- (
+    disj1_tac
+    >> fs[Abbr`P`,DISJ_EQ_IMP,AND_IMP_INTRO]
+    >> rw[same_state_prop_range_def,same_state_prop_def]
+    >> first_x_assum $ qspec_then `LENGTH tr - k` assume_tac
+    >> gs[]
+    >> drule_at (Pat `~parstep_nice _ _ _`) wf_trace_NOT_parstep_nice_state_EQ'
+    >> fs[]
+    >> cheat
+    (* TODO: merge wf_trace1 into wf_trace *)
+  )
+  >> dxrule_then assume_tac arithmeticTheory.WOP
+  >> disj2_tac
+  >> fs[Abbr`P`,DISJ_EQ_IMP,AND_IMP_INTRO]
+  >> qhdtm_x_assum `parstep_nice` $ irule_at Any
+  >> rw[same_state_prop_range_def]
+  >> irule wf_trace_NOT_parstep_nice_same_state_prop
+  >> PRED_ASSUM is_forall $ qspec_then `LENGTH tr - k` assume_tac
+  >> drule_at (Pat `FLOOKUP _ _ = SOME _`) wf_trace_cid_backward
+  >> disch_then $ qspec_then `k` assume_tac
+  >> gs[]
+QED
+*)
+
+(* for a core in a trace either there is previous non-promising progress,
+ * or the core has only made promises *)
+
+Definition only_prom_range_def:
+  only_prom_range cid tr i j <=>
+    i <= j
+    /\ same_state_prop_range cid tr i j (λst. st with <| bst_prom := [] |>)
+    /\ !k. i <= k /\ k < j ==>
+        IS_PREFIX (SND $ EL (SUC k) tr) (SND $ EL k tr)
+        /\ (SND $ EL (SUC k) tr) <> (SND $ EL k tr)
+End
+
+Theorem previous_state_change_non_prom:
+  !i cid tr p st st'.
+  wf_trace tr /\ i < LENGTH tr
+  /\ progressing_trace tr
+  /\ FLOOKUP (FST (EL i tr)) cid = SOME $ Core cid p st
+  ==>
+    only_prom_range cid tr 0 i
+    \/ ?j. j < i
+      /\ parstep_nice cid (EL j tr) (EL (SUC j) tr)
+      /\ (SND $ EL j tr) = (SND $ EL (SUC j) tr)
+      /\ FLOOKUP (FST $ EL j tr) cid = SOME $ Core cid p st
+      /\ FLOOKUP (FST $ EL (SUC j) tr) cid = SOME $ Core cid p st'
+      /\ st with <| bst_prom := [] |> <> st' with <| bst_prom := [] |>
+      /\ only_prom_range cid tr (SUC j) i
+Proof
+  rpt strip_tac
+  >> drule previous_state_change_P
+  >> rpt $ disch_then $ drule_at Any
+  >> disch_then $ qspec_then `λcid tr i j. only_prom_range cid tr i j` mp_tac
+  >> impl_tac
+  >- (
+    fs[prev_state_P_def,only_prom_range_def]
+    >> ntac 3 strip_tac
+    >> dxrule_then strip_assume_tac $ iffLR LESS_OR_EQ
+    >> gs[]
+    >- (
+      conj_tac
+      >- (
+        rw[same_state_prop_range_def,same_state_prop_def]
+        >> first_x_assum drule
+        >> fs[]
+        >> qmatch_goalsub_abbrev_tac `(A ==> _) ==> _`
+        >> Cases_on `A`
+        >- simp[same_state_prop_range_def,same_state_prop_def,LESS_OR_EQ,LEFT_AND_OVER_OR]
+        >> fs[]
+        >> drule_at (Pat `~parstep_nice _ _ _`) wf_trace_NOT_parstep_nice_state_EQ'
+        >> fs[]
+      )
+      >> rw[]
+      >> first_x_assum drule
+      >> fs[]
+      >> qmatch_goalsub_abbrev_tac `(A ==> _) ==> _`
+      >> Cases_on `A`
+      >- simp[same_state_prop_range_def,same_state_prop_def,LESS_OR_EQ,LEFT_AND_OVER_OR]
+      >> fs[]
+      >> cheat (*  *)
+    )
+    >> first_x_assum $ drule_at Any
+    >> fs[]
+    >- (
+      fs[same_state_prop_range_def,same_state_prop_def,PULL_FORALL,AND_IMP_INTRO]
+      >> rpt strip_tac
+
+    )
+  )
+  >> rw[]
+  >> fs[]
+  >> disj2_tac
+  >> goal_assum $ drule_at Any
+  >> fs[]
+  
+QED
+
+(*
+ * characterisation of fulfil and promise rules
+ *)
+
+Definition is_fulfil_def:
+  is_fulfil cid t sys1mem sys2 =
+  ?st st' p a_e v_e xcl acq rel.
+    FLOOKUP (FST sys1mem) cid = SOME $ Core cid p st
+    /\ FLOOKUP sys2 cid = SOME $ Core cid p st'
+    /\ FILTER (λt'. t' <> t) st.bst_prom = st'.bst_prom
+    /\ MEM t st.bst_prom
+    /\ bir_get_stmt (p:string bir_program_t) st.bst_pc = BirStmt_Write a_e v_e xcl acq rel
+    /\ t < (LENGTH $ SND $ sys1mem) + 1
+    /\ 0 < t
+    /\ (EL (PRE t) $ SND $ sys1mem).cid = cid
+End
+
+Theorem is_fulfil_MEM_bst_prom:
+  !cid t sys1 sys2. is_fulfil cid t sys1 sys2
+  ==> ?p st. FLOOKUP (FST sys1) cid = SOME $ Core cid p st /\ MEM t st.bst_prom
+Proof
+  fs[is_fulfil_def,PULL_EXISTS]
+QED
+
+Definition is_promise_def:
+  is_promise cid t sys1 sys2 =
+  ?st st' p v l.
+    FLOOKUP (FST sys1) cid = SOME $ Core cid p st
+    /\ FLOOKUP (FST sys2) cid = SOME $ Core cid p st'
+    /\ t = LENGTH (SND sys1) + 1
+    /\ (SND sys2) = (SND sys1) ++ [<| loc := l; val := v; cid := cid  |>]
+    /\ st'.bst_prom = st.bst_prom ++ [t]
+End
+
+Theorem is_promise_FLOOKUP:
+  !cid t sys1 sys2. is_promise cid t sys1 sys2
+  ==> ?p st. FLOOKUP (FST sys1) cid = SOME $ Core cid p st
+Proof
+  fs[is_promise_def,PULL_EXISTS]
+QED
+
+Theorem is_promise_positive:
+  is_promise cid t sys1 sys2 ==> 0 < t
+Proof
+  fs[is_promise_def,PULL_EXISTS]
+QED
+
+(* amo transition *)
+
+Definition is_amo_def:
+  is_amo cid t sys1mem sys2 =
+  ?st st' p var a_e v_e acq rel.
+    FLOOKUP (FST sys1mem) cid = SOME $ Core cid p st
+    /\ FLOOKUP sys2 cid = SOME $ Core cid p st'
+    /\ FILTER (λt'. t' <> t) st.bst_prom = st'.bst_prom
+    /\ MEM t st.bst_prom
+    /\ bir_get_stmt (p:string bir_program_t) st.bst_pc = BirStmt_Amo var a_e v_e acq rel
+    /\ t < (LENGTH $ SND $ sys1mem) + 1
+    /\ 0 < t
+    /\ (EL (PRE t) $ SND $ sys1mem).cid = cid
+End
+
+(* fulfil steps change the state *)
+
+Theorem is_fulfil_state_changed:
+  !tr cid t p st st' i. wf_trace tr /\ SUC i < LENGTH tr
+  /\ is_fulfil cid t (EL i tr) (FST $ EL (SUC i) tr)
+  /\ FLOOKUP (FST $ EL i tr) cid = SOME $ Core cid p st
+  /\ FLOOKUP (FST $ EL (SUC i) tr) cid = SOME $ Core cid p st'
+  ==> st <> st'
+Proof
+  rpt strip_tac >> gvs[is_fulfil_def]
+  >> qpat_x_assum `MEM _ _` mp_tac
+  >> fs[]
+  >> qpat_x_assum `FILTER _ _ = _` $ ONCE_REWRITE_TAC o single o GSYM
+  >> fs[MEM_FILTER]
+QED
+
+(* promising steps change the state *)
+
+Theorem is_promise_state_changed:
+  !tr cid t p st st' i. wf_trace tr /\ SUC i < LENGTH tr
+  /\ is_promise cid t (EL i tr) (EL (SUC i) tr)
+  /\ FLOOKUP (FST $ EL i tr) cid = SOME $ Core cid p st
+  /\ FLOOKUP (FST $ EL (SUC i) tr) cid = SOME $ Core cid p st'
+  ==> st <> st'
+Proof
+  rpt strip_tac
+  >> gvs[is_promise_def]
+QED
+
+(* parstep and fulfil transitions have same ids *)
+
+Theorem is_fulfil_parstep_nice:
+  !tr i cid cid' t. wf_trace tr /\ SUC i < LENGTH tr
+  /\ progressing_trace tr
+  /\ is_fulfil cid t (EL i tr) (FST $ EL (SUC i) tr)
+  /\ parstep_nice cid' (EL i tr) (EL (SUC i) tr)
+  ==> cid = cid'
+Proof
+  rpt strip_tac
+  >> `parstep_nice cid (EL i tr) (EL (SUC i) tr)` by (
+    CCONTR_TAC
+    >> fs[is_fulfil_def]
+    >> drule_at Any wf_trace_NOT_parstep_nice_state_EQ'
+    >> rpt $ disch_then drule
+    >> disch_then $ fs o single
+    >> drule_at Any FILTER_NEQ_NOT_MEM
+    >> fs[EQ_SYM_EQ]
+  )
+  >> dxrule_all_then irule progressing_trace_cid_eq
+QED
+
+Theorem is_fulfil_parstep_nice_imp:
+  !tr i cid t. wf_trace tr /\ SUC i < LENGTH tr
+  /\ progressing_trace tr
+  /\ is_fulfil cid t (EL i tr) (FST $ EL (SUC i) tr)
+  ==> parstep_nice cid (EL i tr) (EL (SUC i) tr)
+Proof
+  rpt strip_tac
+  >> drule_all_then strip_assume_tac wf_trace_parstep_EL
+  >> drule_all is_fulfil_parstep_nice
+  >> fs[]
+QED
+
+Theorem is_fulfil_memory:
+  !tr i cid t. wf_trace tr /\ SUC i < LENGTH tr
+  /\ progressing_trace tr
+  /\ is_fulfil cid t (EL i tr) (FST $ EL (SUC i) tr)
+  ==> SND $ EL i tr = SND $ EL (SUC i) tr
+Proof
+  rpt strip_tac
+  >> imp_res_tac is_fulfil_parstep_nice_imp
+  >> gvs[parstep_nice_def,parstep_cases,cstep_cases,FLOOKUP_UPDATE,is_fulfil_def]
+  >> `MEM t $ FILTER ($<> t) s.bst_prom` by fs[EQ_SYM_EQ]
+  >> fs[MEM_FILTER]
+QED
+
+Theorem is_fulfil_parstep_nice_eq:
+  !tr cid t i. wf_trace tr /\ SUC i < LENGTH tr
+    /\ progressing_trace tr
+    /\ is_fulfil cid t (EL i tr) (FST $ EL (SUC i) tr)
+    ==>  ?p s var xcl e v_e v_data v_addr v l new_viewenv new_env a_e rel_acq rel acq.
+      bir_get_stmt p s.bst_pc = BirStmt_Write a_e v_e xcl acq rel
+    /\ xcl = is_xcl_write p s.bst_pc
+    /\ rel = is_rel p s.bst_pc
+    /\ acq = is_acq p s.bst_pc
+    /\ rel_acq = (rel /\ acq)
+    /\  MEM t s.bst_prom
+    /\  bir_get_current_statement p s.bst_pc =
+        SOME (BStmtB (BStmt_Assign var e))
+    /\  get_fulfil_args e = SOME (a_e,v_e)
+    /\  oEL (PRE t) (SND (EL (SUC i) tr)) = SOME $ <|loc := l; val := v; cid := cid|>
+    /\  (xcl ==> fulfil_atomic_ok (SND (EL (SUC i) tr)) l cid s t)
+    /\  t < LENGTH (SND (EL (SUC i) tr)) + 1
+    /\  (SOME v,v_data) = bir_eval_exp_view v_e s.bst_environ s.bst_viewenv
+    /\  (SOME l,v_addr) = bir_eval_exp_view a_e s.bst_environ s.bst_viewenv
+    /\  (if acq /\ rel /\ xcl then s.bst_v_Rel else 0) < t
+    /\  (if rel then MAX s.bst_v_rOld s.bst_v_wOld else 0) < t
+    /\  SOME new_viewenv =
+        fulfil_update_viewenv p s xcl t
+    /\  (if xcl then get_xclb_view s.bst_xclb else 0) < t
+    /\  SOME new_env = fulfil_update_env p s xcl
+    /\  s.bst_coh l < t
+    /\  s.bst_v_wNew < t
+    /\  s.bst_v_CAP < t
+    /\  v_data < t
+    /\  v_addr < t
+    /\  FST (EL (SUC i) tr) =
+        FST (EL i tr) |+
+        (cid,
+         Core cid p
+           (s with
+        <|bst_pc :=
+            if is_xcl_write p s.bst_pc then
+              bir_pc_next (bir_pc_next (bir_pc_next s.bst_pc))
+            else bir_pc_next s.bst_pc; bst_environ := new_env;
+          bst_viewenv := new_viewenv;
+          bst_coh :=
+            (\lo. if lo = l then MAX (s.bst_coh l) t else s.bst_coh lo);
+          bst_v_wOld := MAX s.bst_v_wOld t;
+          bst_v_rNew :=
+            if
+              is_acq p s.bst_pc /\ is_rel p s.bst_pc /\
+              is_xcl_write p s.bst_pc
+            then
+              MAX s.bst_v_rNew t
+            else s.bst_v_rNew;
+          bst_v_wNew :=
+            if
+              is_acq p s.bst_pc /\ is_rel p s.bst_pc /\
+              is_xcl_write p s.bst_pc
+            then
+              MAX s.bst_v_wNew t
+            else s.bst_v_wNew; bst_v_CAP := MAX s.bst_v_CAP v_addr;
+          bst_v_Rel :=
+            MAX s.bst_v_Rel
+              (if is_acq p s.bst_pc /\ is_rel p s.bst_pc then t else 0);
+          bst_prom updated_by FILTER (\t'. t' <> t);
+          bst_fwdb :=
+            (\lo.
+                 if lo = l then
+                   <|fwdb_time := t; fwdb_view := MAX v_addr v_data;
+                     fwdb_xcl := is_xcl_write p s.bst_pc|>
+                 else s.bst_fwdb lo);
+          bst_xclb := if is_xcl_write p s.bst_pc then NONE else s.bst_xclb|>))
+    /\  FLOOKUP (FST (EL i tr)) cid = SOME (Core cid p s)
+Proof
+  rpt strip_tac
+  >> drule_all_then assume_tac is_fulfil_parstep_nice_imp
+  >> drule_all_then assume_tac is_fulfil_memory
+  >> gvs[is_fulfil_def,parstep_nice_def,parstep_cases,clstep_cases,cstep_cases,is_fulfil_def,FLOOKUP_UPDATE,bir_programTheory.bir_state_t_accfupds,stmt_generic_step_def,bir_get_stmt_branch,bir_get_stmt_generic,FILTER_EQ_ID,EVERY_MEM,AC CONJ_ASSOC CONJ_COMM,FUPD11_SAME_KEY_AND_BASE,PRE_SUB1]
+  >- (
+    dxrule_at_then Any (drule_at Any) FILTER_NEQ_MEM_EQ
+    >> impl_tac
+    >- (
+      CONV_TAC $ RATOR_CONV $ ONCE_DEPTH_CONV SYM_CONV
+      >> CONV_TAC $ RAND_CONV $ ONCE_DEPTH_CONV SYM_CONV
+      >> fs[]
+    )
+    >> disch_then $ fs o single
+    >> gvs[bir_get_stmt_write]
+    >> rpt $ goal_assum $ rev_drule_at Any
+    >> fs[]
+  )
+  >> gs[bir_get_stmt_write,stmt_generic_step_def]
+QED
+
+(* parstep and promise transitions have same ids *)
+
+Theorem is_promise_parstep_nice:
+  !tr i cid cid' t. wf_trace tr /\ SUC i < LENGTH tr
+  /\ is_promise cid t (EL i tr) (EL (SUC i) tr)
+  /\ parstep_nice cid' (EL i tr) (EL (SUC i) tr)
+  ==> cid = cid'
+Proof
+  rpt strip_tac
+  >> fs[parstep_nice_def,parstep_cases,cstep_cases,clstep_cases,is_promise_def]
+  >> gvs[]
+QED
+
+Theorem is_promise_parstep_nice_imp:
+  !tr i cid t. wf_trace tr /\ SUC i < LENGTH tr
+  /\ is_promise cid t (EL i tr) (EL (SUC i) tr)
+  ==> parstep_nice cid (EL i tr) (EL (SUC i) tr)
+Proof
+  rpt strip_tac
+  >> drule_all_then strip_assume_tac wf_trace_parstep_EL
+  >> drule_all is_promise_parstep_nice
+  >> fs[]
+QED
+
+Theorem is_promise_parstep_nice_eq:
+  !tr i cid t. wf_trace tr /\ SUC i < LENGTH tr
+  /\ is_promise cid t (EL i tr) (EL (SUC i) tr)
+  ==> ?msg p s. cid = msg.cid
+    /\ FLOOKUP (FST (EL i tr)) cid = SOME (Core cid p s)
+    /\  SND (EL (SUC i) tr) = SND (EL i tr) ⧺ [msg]
+    /\  FST (EL (SUC i) tr) =
+        FST (EL i tr) |+
+        (cid,
+          Core cid p
+            (s with
+            bst_prom updated_by (λpr. pr ⧺ [LENGTH (SND (EL i tr)) + 1])))
+    /\  atomicity_ok cid (FST (EL i tr))
+    /\  is_certified p cid
+          (s with
+            bst_prom updated_by (λpr. pr ⧺ [LENGTH (SND (EL i tr)) + 1]))
+          (SND (EL i tr) ⧺ [msg])
+Proof
+  rpt strip_tac
+  >> imp_res_tac is_promise_parstep_nice_imp
+  >> fs[parstep_nice_def,parstep_cases,cstep_cases,clstep_cases,is_promise_def]
+  >> gvs[]
+QED
+
+(* fulfil steps affect only the fulfiling core *)
+
+Theorem is_fulfil_inv:
+  !tr cid cid' t p p2 p2' st st' st2 st2' i.
+  wf_trace tr /\ SUC i < LENGTH tr
+  /\ is_fulfil cid t (EL i tr) (FST $ EL (SUC i) tr)
+  /\ FLOOKUP (FST $ EL i tr) cid = SOME $ Core cid p st
+  /\ FLOOKUP (FST $ EL (SUC i) tr) cid = SOME $ Core cid p st'
+  /\ FLOOKUP (FST $ EL i tr) cid' = SOME $ Core cid' p2 st2
+  /\ FLOOKUP (FST $ EL (SUC i) tr) cid' = SOME $ Core cid' p2' st2'
+  /\ cid <> cid'
+  ==> st <> st' /\ p2 = p2' /\ st2 = st2'
+Proof
+  rpt gen_tac >> strip_tac
+  >> conj_asm1_tac
+  >- (
+    drule_then irule is_fulfil_state_changed
+    >> rpt $ goal_assum $ drule_at Any
+  )
+  >>  drule_then (drule_then irule) wf_trace_unchanged
+  >> rpt $ goal_assum $ drule_at Any
+QED
+
+(* promise steps affect only the promising core *)
+
+Theorem is_promise_inv:
+  !tr cid cid' t p p2 p2' st st' st2 st2' i.
+  wf_trace tr /\ SUC i < LENGTH tr
+  /\ is_promise cid t (EL i tr) (EL (SUC i) tr)
+  /\ FLOOKUP (FST $ EL i tr) cid = SOME $ Core cid p st
+  /\ FLOOKUP (FST $ EL (SUC i) tr) cid = SOME $ Core cid p st'
+  /\ FLOOKUP (FST $ EL i tr) cid' = SOME $ Core cid' p2 st2
+  /\ FLOOKUP (FST $ EL (SUC i) tr) cid' = SOME $ Core cid' p2' st2'
+  /\ cid <> cid'
+  ==> st <> st' /\ p2 = p2' /\ st2 = st2'
+Proof
+  rpt gen_tac >> strip_tac
+  >> conj_asm1_tac
+  >- (
+    drule_then irule is_promise_state_changed
+    >> rpt $ goal_assum $ drule_at Any
+  )
+  >>  drule_then (drule_then irule) wf_trace_unchanged
+  >> rpt $ goal_assum $ drule_at Any
+QED
+
+(* a promise entails lower bound of future memory length *)
+
+Theorem is_promise_LENGTH_SND_EL:
+  !i j tr cid t. wf_trace tr
+  /\ is_promise cid t (EL i tr) (EL (SUC i) tr)
+  /\ SUC i <= j /\ j < LENGTH tr
+  ==> t <= LENGTH (SND $ EL j tr)
+Proof
+  rpt gen_tac
+  >> Induct_on `j - SUC i`
+  >- (rw[is_promise_def] >> gs[LESS_OR_EQ])
+  >> rw[SUB_LEFT_EQ]
+  >> first_x_assum $ rev_drule_at Any
+  >> disch_then $ rev_drule_at Any
+  >> disch_then $ qspec_then `v + SUC i` assume_tac
+  >> `SUC $ v + SUC i < LENGTH tr` by fs[]
+  >> drule_all_then strip_assume_tac wf_trace_parstep_EL
+  >> dxrule_then strip_assume_tac parstep_nice_memory_imp
+  >> gs[]
+  >> `SUC i + SUC v = SUC $ v + SUC i` by fs[]
+  >> pop_assum $ fs o single
+QED
+
+(* a promise is only promised once *)
+
+Theorem is_promise_once:
+  !i j tr cid cid' t. wf_trace tr
+  /\ is_promise cid t (EL i tr) (EL (SUC i) tr)
+  /\ i < j /\ SUC j < LENGTH tr
+  ==> ~is_promise cid' t (EL j tr) (EL (SUC j) tr)
+Proof
+  rpt strip_tac
+  >> rev_drule_at Any is_promise_LENGTH_SND_EL
+  >> disch_then $ rev_drule_at_then Any assume_tac
+  >> first_assum $ qspec_then `j` assume_tac
+  >> first_x_assum $ qspec_then `SUC j` assume_tac
+  >> dxrule_then strip_assume_tac $ iffLR is_promise_def
+  >> gvs[]
+QED
+
+(* a fulfil has an earlier promise *)
+
+Theorem NOT_is_promise_NOT_MEM_bst_prom:
+  !i tr cid p st st' t. wf_trace tr
+  /\ ~is_promise cid t (EL i tr) (EL (SUC i) tr)
+  /\ SUC i < LENGTH tr
+  /\ FLOOKUP (FST $ EL i tr) cid = SOME $ Core cid p st
+  /\ ~MEM t st.bst_prom
+  /\ FLOOKUP (FST $ EL (SUC i) tr) cid = SOME $ Core cid p st'
+  ==> ~MEM t st'.bst_prom
+Proof
+  rw[]
+  >> drule_all_then strip_assume_tac wf_trace_parstep_EL
+  >> Cases_on `cid = cid'`
+  >- (
+    BasicProvers.VAR_EQ_TAC
+    >> fs[is_promise_def,DISJ_EQ_IMP]
+    >> fs[AND_IMP_INTRO,AC CONJ_ASSOC CONJ_COMM,cstep_cases,parstep_nice_def,parstep_cases]
+    (* execute *)
+    >- (
+      imp_res_tac clstep_LENGTH_prom
+      >> gvs[FLOOKUP_UPDATE]
+      >- (imp_res_tac clstep_bst_prom_EQ >> fs[])
+      >> gvs[clstep_cases,MEM_FILTER,FLOOKUP_UPDATE]
+    )
+    (* promises *)
+    >> spose_not_then assume_tac
+    >> gvs[FLOOKUP_UPDATE,mem_msg_t_component_equality]
+  )
+  >> gs[parstep_nice_def,parstep_cases,FLOOKUP_UPDATE]
+QED
+
+Theorem is_fulfil_is_promise:
+  !i tr cid t. wf_trace tr /\ SUC i < LENGTH tr
+  /\ is_fulfil cid t (EL i tr) (FST $ EL (SUC i) tr)
+  ==> ?j. j < i /\ is_promise cid t (EL j tr) (EL (SUC j) tr)
+Proof
+  rpt strip_tac
+  >> CCONTR_TAC
+  >> fs[DISJ_EQ_IMP]
+  >> `!j p st. j <= i /\ FLOOKUP (FST $ EL j tr) cid = SOME $ Core cid p st
+    ==> ~MEM t st.bst_prom` by (
+    Induct
+    >- (
+      rw[] >> fs[wf_trace_def,empty_prom_def]
+      >> strip_tac
+      >> res_tac
+      >> gs[NULL_EQ]
+    )
+    >> rw[] >> gs[]
+    >> `j < i` by fs[]
+    >> first_x_assum $ dxrule_then assume_tac
+    >> drule_then drule wf_trace_cid_backward1
+    >> rw[]
+    >> first_x_assum $ drule_then assume_tac
+    >> drule_then drule NOT_is_promise_NOT_MEM_bst_prom
+    >> rpt $ disch_then $ drule_at Any
+    >> fs[]
+  )
+  >> fs[is_fulfil_def]
+  >> first_x_assum $ rev_drule_at Any
+  >> fs[]
+QED
+
+(* a promise has a succeeding fulfil *)
+
+Theorem NOT_is_fulfil_MEM_bst_prom:
+  !i tr cid p st p' st' t. wf_trace tr /\ SUC i < LENGTH tr
+  /\ ~is_fulfil cid t (EL i tr) (FST $ EL (SUC i) tr)
+  /\ ~is_amo cid t (EL i tr) (FST $ EL (SUC i) tr)
+  /\ FLOOKUP (FST $ EL i tr) cid = SOME $ Core cid p st
+  /\ MEM t st.bst_prom
+  /\ FLOOKUP (FST $ EL (SUC i) tr) cid = SOME $ Core cid p st'
+  ==> MEM t st'.bst_prom
+Proof
+  rw[]
+  >> drule_all_then strip_assume_tac wf_trace_parstep_EL
+  >> fs[parstep_nice_def,parstep_cases,DISJ_EQ_IMP,is_fulfil_def,is_amo_def]
+  >> Cases_on `cid = cid'`
+  >> gvs[FLOOKUP_UPDATE,DISJ_EQ_IMP]
+  >> fs[AND_IMP_INTRO,AC CONJ_ASSOC CONJ_COMM,cstep_cases,parstep_nice_def,parstep_cases]
+  >> imp_res_tac clstep_LENGTH_prom
+  >> gvs[FLOOKUP_UPDATE,oEL_THM]
+  >- (imp_res_tac clstep_bst_prom_EQ >> fs[])
+  >> spose_not_then assume_tac
+  >> gvs[clstep_cases,MEM_FILTER,FLOOKUP_UPDATE,PRE_SUB1,oEL_THM]
+QED
+
+Theorem is_promise_is_fulfil:
+  !i tr cid t. wf_trace tr /\ SUC i < LENGTH tr
+  /\ is_promise cid t (EL i tr) (EL (SUC i) tr)
+  ==> ?j. i < j /\ SUC j < LENGTH tr
+    /\ (is_fulfil cid t (EL j tr) (FST $ EL (SUC j) tr)
+    \/ is_amo cid t (EL j tr) (FST $ EL (SUC j) tr))
+Proof
+  rpt strip_tac
+  >> CCONTR_TAC
+  >> fs[DISJ_EQ_IMP]
+  >> `!j p st. i <= j /\ SUC j < LENGTH tr
+    /\ FLOOKUP (FST $ EL (SUC j) tr) cid = SOME $ Core cid p st
+    ==> MEM t st.bst_prom` by (
+    Induct_on `j - i`
+    >- (rw[] >> gvs[LESS_OR_EQ,is_promise_def,FLOOKUP_UPDATE])
+    >> rw[SUB_LEFT_EQ] >> fs[]
+    >> first_x_assum $ qspecl_then [`i + v`,`i`] mp_tac
+    >> fs[]
+    >> `?st. FLOOKUP (FST $ EL (SUC $ i + v) tr) cid = SOME $ Core cid p st` by (
+      irule wf_trace_cid_backward1
+      >> `SUC $ i + SUC v = SUC $ SUC $ i + v` by fs[]
+      >> pop_assum $ fs o single
+    )
+    >> disch_then $ drule_then assume_tac
+    >> drule NOT_is_fulfil_MEM_bst_prom
+    >> rpt $ disch_then $ drule_at Any
+    >> disch_then irule
+    >> fs[]
+    >> `SUC $ i + SUC v = SUC $ SUC $ i + v` by fs[]
+    >> pop_assum $ fs o single
+  )
+  >> `?p st. FLOOKUP (FST $ LAST tr) cid = SOME $ Core cid p st` by (
+    fs[is_promise_def,GSYM LENGTH_NOT_NULL,GSYM NULL_EQ,LAST_EL]
+    >> qexists_tac `p`
+    >> drule_then irule wf_trace_cid_forward
+    >> fs[]
+    >> goal_assum $ drule_at Any
+    >> fs[]
+  )
+  >> drule_all wf_trace_LAST_NULL_bst_prom
+  >> gs[GSYM LENGTH_NOT_NULL,GSYM NULL_EQ,LAST_EL]
+  >> Cases_on `SUC i = PRE $ LENGTH tr`
+  >- fs[is_promise_def]
+  >> gs[NOT_NUM_EQ]
+  >> `i <= PRE $ PRE $ LENGTH tr` by fs[]
+  >> first_x_assum dxrule
+  >> `0 < PRE $ LENGTH tr` by fs[]
+  >> fs[iffLR SUC_PRE]
+  >> rw[LENGTH_NOT_NULL,MEM_SPLIT,NOT_NULL_MEM]
+  >> goal_assum drule
+QED
+
+(* every addition to memory is a promise *)
+
+Theorem wf_trace_EL_SND_is_promise:
+  !i tr k. wf_trace tr /\ i < LENGTH tr
+  /\ k < LENGTH $ SND $ EL i tr
+  ==> ?j. j < i
+    /\ is_promise (EL k $ SND $ EL i tr).cid (SUC k) (EL j tr) (EL (SUC j) tr)
+Proof
+  rpt strip_tac
+  >> qmatch_goalsub_abbrev_tac `is_promise cid _ _`
+  >> drule wf_trace_adds_to_memory
+  >> rpt $ disch_then drule
+  >> disch_then $ qspec_then `cid` assume_tac
+  >> fs[Abbr`cid`]
+  >> goal_assum drule
+  >> gs[is_promise_def,FLOOKUP_UPDATE,parstep_nice_def,parstep_cases,cstep_cases,mem_msg_t_component_equality]
+QED
+
+(* the timestamp of a fulfil is coupled to the fulfiled core *)
+
+Theorem is_fulfil_to_memory:
+  !tr i cid t. wf_trace tr /\ SUC i < LENGTH tr
+  /\ progressing_trace tr
+  /\ is_fulfil cid t (EL i tr) (FST $ EL (SUC i) tr)
+  ==> 0 < t /\ t < (LENGTH $ SND $ EL (SUC i) tr) + 1
+    /\ (EL (PRE t) $ SND $ EL (SUC i) tr).cid = cid
+Proof
+  rpt gen_tac >> strip_tac
+  >> drule_all_then strip_assume_tac is_fulfil_parstep_nice_eq
+  >> gs[arithmeticTheory.PRE_SUB1,oEL_THM]
+QED
+
+(* a fulfil is only fulfilled once *)
+
+Theorem is_fulfil_once:
+  !tr i j t cid cid'. wf_trace tr
+  /\ progressing_trace tr
+  /\ SUC i < LENGTH tr
+  /\ is_fulfil cid t (EL i tr) (FST $ EL (SUC i) tr)
+  /\ SUC j < LENGTH tr /\ i <> j
+  ==> ~is_fulfil cid' t (EL j tr) (FST $ EL (SUC j) tr)
+Proof
+  rpt strip_tac
+  >> wlog_tac `i < j` [`i`,`j`,`cid`,`cid'`]
+  >- metis_tac[NOT_NUM_EQ,LESS_EQ]
+  >> qmatch_assum_rename_tac `is_fulfil cid t (EL i tr) _`
+  >> qmatch_assum_rename_tac `is_fulfil cid' t (EL j tr) _`
+  >> drule_at (Pos $ el 4) is_fulfil_to_memory
+  >> rev_drule_at (Pos $ el 4) is_fulfil_to_memory
+  >> drule_at (Pos $ el 4) is_fulfil_memory
+  >> rev_drule_at (Pos $ el 4) is_fulfil_memory
+  >> rpt strip_tac >> gs[]
+  >> `cid = cid'` by (
+    drule_then (qspecl_then [`SUC i`,`SUC j`] mp_tac) wf_trace_IS_PREFIX_SND_EL
+    >> rw[IS_PREFIX_APPEND]
+    >> fs[EL_APPEND1]
+  )
+  >> gvs[]
+  >> Cases_on `j = SUC i`
+  >> gvs[FLOOKUP_UPDATE,is_fulfil_def]
+  >> drule_then (rev_drule_then $ drule_at Any) wf_trace_cid
+  >> disch_then strip_assume_tac
+  >> gvs[]
+  >- (
+    ntac 2 $ qhdtm_x_assum `FILTER` $ fs o single o GSYM
+    >> fs[MEM_FILTER]
+  )
+  >> qmatch_assum_abbrev_tac `cid = _.cid`
+  >> qspecl_then [`SUC i`,`j`,`tr`,`cid`] assume_tac
+    wf_trace_EVERY_NOT_MEM_bst_prom_LENGTH_LESS_bst_prom
+  >> gs[EVERY_MEM,AND_IMP_INTRO,Abbr`cid`]
+  >> first_x_assum drule
+  >> impl_tac
+  >- (
+    ntac 2 $ qhdtm_x_assum `FILTER` $ fs o single o GSYM
+    >> fs[MEM_FILTER]
+  )
+  >> fs[NOT_LESS]
+QED
+
+(* only one fulfil happens at a time *)
+
+Theorem is_fulfil_same:
+  !tr cid cid' t t' i. wf_trace tr
+  /\ progressing_trace tr
+  /\ is_fulfil cid t (EL i tr) (FST $ EL (SUC i) tr)
+  /\ is_fulfil cid' t' (EL i tr) (FST $ EL (SUC i) tr)
+  /\ SUC i < LENGTH tr
+  ==> cid = cid' /\ t = t'
+Proof
+  rpt gen_tac >> strip_tac
+  >> conj_asm1_tac
+  >- (
+    drule_at_then (Pat `is_fulfil _ _ _ _`) assume_tac is_fulfil_parstep_nice_imp
+    >> rev_drule_at_then (Pat `is_fulfil _ _ _ _`) assume_tac is_fulfil_parstep_nice_imp
+    >> gs[]
+    >> dxrule_at_then Any irule progressing_trace_cid_eq
+    >> fs[]
+  )
+  >> gvs[is_fulfil_def]
+  >> qhdtm_x_assum `FILTER` $ fs o single o GSYM
+  >> dxrule_at_then Any (dxrule_at Any) FILTER_NEQ_MEM_EQ
+  >> fs[EQ_SYM_EQ]
+QED
+
+(* only one promise happens at a time *)
+
+Theorem is_promise_same:
+  !tr cid cid' t t' i. wf_trace tr
+  /\ is_promise cid t (EL i tr) (EL (SUC i) tr)
+  /\ is_promise cid' t' (EL i tr) (EL (SUC i) tr)
+  /\ SUC i < LENGTH tr
+  ==> cid = cid' /\ t = t'
+Proof
+  rpt gen_tac >> strip_tac
+  >> conj_asm1_tac
+  >- gvs[is_promise_def]
+  >> fs[is_promise_def]
+QED
+
+(* For a thread cid, the coh(l) of an address l fulfiled to is strictly larger than t *)
+Theorem is_fulfil_bst_coh:
+  !tr i j cid t p st. wf_trace tr
+  /\ progressing_trace tr
+  /\ is_fulfil cid t (EL i tr) (FST $ EL (SUC i) tr)
+  /\ i < j /\ j < LENGTH tr
+  /\ FLOOKUP (FST $ EL j tr) cid = SOME $ Core cid p st
+  ==> t < st.bst_coh((EL t $ SND $ EL (SUC i) tr).loc)
+Proof
+  rpt gen_tac
+  >> Induct_on `j - i` >> fs[]
+  >> rw[SUB_LEFT_EQ]
+  >> first_x_assum $ qspecl_then [`v + i`,`i`] assume_tac
+  >> Cases_on `0 < v`
+  >> gs[]
+  >- (
+    cheat
+  )
+  >> drule_at_then (Pos $ el 3) assume_tac is_fulfil_parstep_nice_imp
+  >> drule_at_then (Pos $ el 3) assume_tac is_fulfil_to_memory
+  >> gvs[parstep_nice_def,parstep_cases,FLOOKUP_UPDATE]
+  >> cheat
+QED
+
+(* the fulfiling core location *)
+
+Theorem is_fulfil_promise_loc:
+  !tr i cid t p st st' a_e v_e xcl acq rel l v_addr .
+  wf_trace tr /\ SUC i < LENGTH tr
+  /\ progressing_trace tr
+  /\ is_fulfil cid t (EL i tr) (FST $ EL (SUC i) tr)
+  /\ FLOOKUP (FST $ EL i tr) cid = SOME $ Core cid p st
+  /\ bir_get_stmt p st.bst_pc = BirStmt_Write a_e v_e xcl acq rel
+  /\ bir_eval_exp_view a_e st.bst_environ st.bst_viewenv = (SOME l,v_addr)
+  ==> PRE t < LENGTH (SND (EL i tr))
+    /\ cid = (EL (PRE t) $ SND $ EL i tr).cid
+    /\ l = (EL (PRE t) $ SND $ EL i tr).loc
+Proof
+  rpt gen_tac >> strip_tac
+  >> drule_all_then strip_assume_tac is_fulfil_is_promise
+  >> qmatch_assum_rename_tac `j < i`
+  >> `IS_PREFIX (SND $ EL i tr) (SND $ EL (SUC j) tr)` by (
+    dxrule_then assume_tac $ iffLR LESS_EQ
+    >> gvs[LESS_OR_EQ]
+    >> irule wf_trace_IS_PREFIX_SND_EL
+    >> fs[]
+  )
+  >> imp_res_tac is_promise_positive
+  >> drule_all_then strip_assume_tac is_fulfil_memory
+  >> gvs[is_promise_def,FLOOKUP_UPDATE,IS_PREFIX_APPEND,EL_APPEND2,SUC_PRE,GSYM ADD1]
+  >> drule_all_then strip_assume_tac is_fulfil_parstep_nice_eq
+  >> gvs[FLOOKUP_UPDATE,EL_APPEND1,oEL_THM]
+QED
+
+(*
+ * exclusive reads and stores
+ *)
+
+Definition is_read_xcl_def:
+  is_read_xcl cid t sys1mem sys2 <=>
+  ?st st' p var a_e cast_opt acq rel.
+    FLOOKUP (FST sys1mem) cid = SOME $ Core cid p st
+    /\ FLOOKUP sys2 cid = SOME $ Core cid p st'
+    /\ bir_get_stmt p st.bst_pc = BirStmt_Read var a_e cast_opt T acq rel
+    /\ IS_SOME st'.bst_xclb
+    /\ (THE st'.bst_xclb).xclb_time = t
+    /\ IS_NONE st.bst_xclb
+    /\ (0 < t
+      ==>
+        PRE t < LENGTH $ SND sys1mem
+        /\ (EL (PRE t) $ SND sys1mem).cid = cid)
+End
+
+Definition is_fulfil_xcl_def:
+  is_fulfil_xcl cid t sys1mem sys2 <=>
+  ?st st' p a_e v_e acq rel.
+    FLOOKUP (FST sys1mem) cid = SOME $ Core cid p st
+    /\ FLOOKUP sys2 cid = SOME $ Core cid p st'
+    /\ FILTER (λt'. t' <> t) st.bst_prom = st'.bst_prom
+    /\ MEM t st.bst_prom
+    /\ bir_get_stmt (p:string bir_program_t) st.bst_pc
+      = BirStmt_Write a_e v_e T acq rel
+    /\ IS_SOME st.bst_xclb
+    /\ PRE t < LENGTH $ SND $ sys1mem
+    /\ 0 < t
+    /\ (EL (PRE t) $ SND $ sys1mem).cid = cid
+End
+
+Theorem is_fulfil_xcl_is_fulfil:
+  !cid t sys1mem sys2. is_fulfil_xcl cid t sys1mem sys2
+  ==> is_fulfil cid t sys1mem sys2
+Proof
+  rw[is_fulfil_xcl_def,is_fulfil_def,bir_get_stmt_write]
+  >> rpt $ goal_assum $ drule_at Any
+QED
+
+(* an exclusive fulfil does not affect fwdb of other locations *)
+
+Theorem is_fulfil_xcl_bst_fwdb_eq:
+  !tr i cid p st st' l t. wf_trace tr /\ SUC i < LENGTH tr
+  /\ progressing_trace tr
+  /\ is_fulfil_xcl cid t (EL i tr) (FST $ EL (SUC i) tr)
+  /\ l <> (EL (PRE t) $ SND $ EL i tr).loc
+  /\ FLOOKUP (FST $ EL i tr) cid = SOME $ Core cid p st
+  /\ FLOOKUP (FST $ EL (SUC i) tr) cid = SOME $ Core cid p st'
+  ==> st.bst_fwdb l = st'.bst_fwdb l
+Proof
+  rpt strip_tac
+  >> imp_res_tac is_fulfil_xcl_is_fulfil
+  >> drule_at_then (Pat `is_fulfil _ _ _ _`) assume_tac is_fulfil_promise_loc
+  >> gvs[]
+  >> dxrule_at_then (Pat `is_fulfil _ _ _ _`) assume_tac is_fulfil_parstep_nice_eq
+  >> gvs[FLOOKUP_UPDATE]
+  >> ntac 2 $ qpat_x_assum `_ = bir_eval_exp_view _ _ _` $ assume_tac o GSYM
+  >> gvs[]
+QED
+
+Theorem is_fulfil_xcl_atomic:
+  !tr i cid t p st.  wf_trace tr /\ SUC i < LENGTH tr
+  /\ progressing_trace tr
+  /\ is_fulfil_xcl cid t (EL i tr) (FST $ EL (SUC i) tr)
+  /\ FLOOKUP (FST $ EL i tr) cid = SOME $ Core cid p st
+  ==> fulfil_atomic_ok (SND $ EL (SUC i) tr)
+        ((EL (PRE t) $ SND $ EL (SUC i) tr).loc) cid st t
+    /\ is_xcl_write p st.bst_pc
+    /\  (EL (PRE t) $ SND $ EL (SUC i) tr).cid = cid
+Proof
+  rpt gen_tac >> strip_tac
+  >> imp_res_tac is_fulfil_xcl_is_fulfil
+  >> drule_at_then Any assume_tac is_fulfil_parstep_nice_eq
+  >> gvs[is_fulfil_xcl_def,bir_get_stmt_write,oEL_THM]
+QED
+
+(* parstep and read transitions have same ids *)
+
+Theorem is_read_xcl_parstep_nice:
+  !tr i cid cid' t. wf_trace tr /\ SUC i < LENGTH tr
+  /\ progressing_trace tr
+  /\ is_read_xcl cid t (EL i tr) (FST $ EL (SUC i) tr)
+  /\ parstep_nice cid' (EL i tr) (EL (SUC i) tr)
+  ==> cid = cid'
+Proof
+  rpt strip_tac
+  >> `parstep_nice cid (EL i tr) (EL (SUC i) tr)` by (
+    CCONTR_TAC
+    >> fs[is_read_xcl_def]
+    >> drule_at Any wf_trace_NOT_parstep_nice_state_EQ'
+    >> rpt $ disch_then drule
+    >> disch_then $ fs o single
+  )
+  >> dxrule_all progressing_trace_cid_eq
+  >> fs[]
+QED
+
+Theorem is_read_xcl_parstep_nice_imp:
+  !tr i cid t. wf_trace tr /\ SUC i < LENGTH tr
+  /\ progressing_trace tr
+  /\ is_read_xcl cid t (EL i tr) (FST $ EL (SUC i) tr)
+  ==> parstep_nice cid (EL i tr) (EL (SUC i) tr)
+Proof
+  rpt strip_tac
+  >> drule_all_then strip_assume_tac wf_trace_parstep_EL
+  >> dxrule is_read_xcl_parstep_nice
+  >> rpt $ disch_then $ drule_at Any
+  >> fs[]
+QED
+
+(* parstep transition of an exclusive read *)
+
+Theorem is_read_xcl_parstep_nice_eq:
+  !tr cid t i. wf_trace tr /\ SUC i < LENGTH tr
+    /\ progressing_trace tr
+    /\ is_read_xcl cid t (EL i tr) (FST $ EL (SUC i) tr)
+    ==> ?p s st' opt_cast v_pre v_addr new_env l a_e var v zcq rel acq.
+      is_certified p cid st' (SND (EL (SUC i) tr))
+      /\ FST (EL (SUC i) tr) = FST (EL i tr) |+ (cid, Core cid p st')
+      /\ st' = s with
+        <|bst_pc := bir_pc_next (bir_pc_next s.bst_pc);
+          bst_environ := new_env;
+          bst_viewenv updated_by
+            (\env.
+                 env |+
+                 (var,
+                  MAX
+                    (MAX
+                       (MAX (MAX v_addr s.bst_v_rNew)
+                          (if acq /\ rel then s.bst_v_Rel else 0))
+                       (if acq /\ rel then MAX s.bst_v_rOld s.bst_v_wOld
+                        else 0)) (mem_read_view (s.bst_fwdb l) t)));
+          bst_coh :=
+            (\lo.
+                 if lo = l then
+                   MAX (s.bst_coh l)
+                     (MAX
+                        (MAX
+                           (MAX (MAX v_addr s.bst_v_rNew)
+                              (if acq /\ rel then s.bst_v_Rel else 0))
+                           (if acq /\ rel then MAX s.bst_v_rOld s.bst_v_wOld
+                            else 0)) (mem_read_view (s.bst_fwdb l) t))
+                 else s.bst_coh lo);
+          bst_v_rOld :=
+            MAX s.bst_v_rOld
+              (MAX
+                 (MAX
+                    (MAX (MAX v_addr s.bst_v_rNew)
+                       (if acq /\ rel then s.bst_v_Rel else 0))
+                    (if acq /\ rel then MAX s.bst_v_rOld s.bst_v_wOld else 0))
+                 (mem_read_view (s.bst_fwdb l) t));
+          bst_v_rNew :=
+            if acq then
+              MAX s.bst_v_rNew
+                (MAX
+                   (MAX
+                      (MAX (MAX v_addr s.bst_v_rNew)
+                         (if rel then s.bst_v_Rel else 0))
+                      (if rel then MAX s.bst_v_rOld s.bst_v_wOld else 0))
+                   (mem_read_view (s.bst_fwdb l) t))
+            else s.bst_v_rNew;
+          bst_v_wNew :=
+            if acq then
+              MAX s.bst_v_wNew
+                (MAX
+                   (MAX
+                      (MAX (MAX v_addr s.bst_v_rNew)
+                         (if rel then s.bst_v_Rel else 0))
+                      (if rel then MAX s.bst_v_rOld s.bst_v_wOld else 0))
+                   (mem_read_view (s.bst_fwdb l) t))
+            else s.bst_v_wNew; bst_v_CAP := MAX s.bst_v_CAP v_addr;
+          bst_v_Rel :=
+            MAX s.bst_v_Rel
+              (if rel /\ acq then
+                 MAX
+                   (MAX (MAX (MAX v_addr s.bst_v_rNew) s.bst_v_Rel)
+                      (MAX s.bst_v_rOld s.bst_v_wOld))
+                   (mem_read_view (s.bst_fwdb l) t)
+               else 0);
+          bst_xclb :=
+            SOME
+              <|xclb_time := t;
+                xclb_view :=
+                  MAX
+                    (MAX
+                       (MAX (MAX v_addr s.bst_v_rNew)
+                          (if acq /\ rel then s.bst_v_Rel else 0))
+                       (if acq /\ rel then MAX s.bst_v_rOld s.bst_v_wOld
+                        else 0)) (mem_read_view (s.bst_fwdb l) t)|> |>
+      /\ FLOOKUP (FST (EL i tr)) cid = SOME (Core cid p s)
+      /\ atomicity_ok cid (FST (EL i tr))
+      /\ SOME new_env = env_update_cast64 (bir_var_name var) v (bir_var_type var) s.bst_environ
+      /\ (!t'.
+          t < t' /\
+          ((((t' <= v_addr \/ t' <= s.bst_v_rNew) \/
+             t' <= if acq /\ rel then s.bst_v_Rel else 0) \/
+            t' <= if acq /\ rel then MAX s.bst_v_rOld s.bst_v_wOld else 0) \/
+           t' <= s.bst_coh l) ==>
+          ?msg. oEL (t' - 1) (SND (EL i tr)) = SOME msg /\ msg.loc <> l)
+      /\ mem_read (SND (EL i tr)) l t = SOME v
+      /\ (SOME l,v_addr) = bir_eval_exp_view a_e s.bst_environ s.bst_viewenv
+      /\ bir_get_stmt p s.bst_pc = BirStmt_Read var a_e opt_cast T acq rel
+      /\ SND (EL (SUC i) tr) = SND (EL i tr)
+Proof
+  rpt strip_tac
+  >> imp_res_tac is_read_xcl_parstep_nice_imp
+  >> dxrule_then assume_tac $ iffLR parstep_nice_def
+  >> dxrule_then strip_assume_tac $ iffLR parstep_cases
+  >> rpt $ goal_assum $ drule_at Any
+  >> gvs[cstep_cases,clstep_cases,is_read_xcl_def,optionTheory.IS_SOME_EXISTS,is_read_xcl_def,FLOOKUP_UPDATE]
+  >> rpt $ goal_assum $ drule_at Any
+  >> dsimp[bir_programTheory.bir_state_t_component_equality,pairTheory.ELIM_UNCURRY,FUN_EQ_THM,mem_read_view_def]
+QED
+
+Theorem mem_read_EL_SND_loc:
+  !t M l. 0 < t /\ IS_SOME $ mem_read M l t
+  /\ PRE t < LENGTH M
+  ==> l = (EL (PRE t) M).loc
+Proof
+  Cases >> fs[mem_read_def,oEL_THM] >> Induct
+  >> rw[oEL_def,optionTheory.IS_SOME_EXISTS,mem_read_aux_def]
+QED
+
+Theorem is_read_xcl_LENGTH_SND_EL:
+  !t cid i tr. wf_trace tr /\ SUC i < LENGTH tr
+  /\ progressing_trace tr
+  /\ is_read_xcl cid t (EL i tr) (FST $ EL (SUC i) tr)
+  ==> (0 < t ==> PRE t < LENGTH $ SND $ EL i tr)
+    /\ SND $ EL i tr = SND $ EL (SUC i) tr
+Proof
+  Cases >> rpt gen_tac >> strip_tac
+  >> drule_all_then strip_assume_tac is_read_xcl_parstep_nice_eq
+  >> fs[mem_read_def,mem_read_aux_def,oEL_THM]
+  >> qhdtm_x_assum `mem_read_aux` mp_tac
+  >> IF_CASES_TAC
+  >> fs[mem_read_aux_def]
+QED
+
+(* only exclusive loads set the exclusive bank *)
+
+Theorem xclb_NONE_SOME_is_read_xclb:
+  !cid p p' st st' i tr. wf_trace tr /\ SUC i < LENGTH tr
+  /\ FLOOKUP (FST $ EL i tr) cid = SOME $ Core cid p st
+  /\ FLOOKUP (FST $ EL (SUC i) tr) cid = SOME $ Core cid p st'
+  /\ IS_SOME st'.bst_xclb
+  /\ st.bst_xclb = NONE
+  ==> ?t. is_read_xcl cid t (EL i tr) (FST $ EL (SUC i) tr)
+Proof
+  rpt strip_tac
+  >> drule_all_then strip_assume_tac wf_trace_parstep_EL
+  >> fs[parstep_nice_def,parstep_cases,DISJ_EQ_IMP]
+  >> reverse $ Cases_on `cid = cid'`
+  >> gvs[FLOOKUP_UPDATE,clstep_cases,cstep_cases,parstep_nice_def,parstep_cases,is_read_xcl_def,optionTheory.IS_SOME_EXISTS]
+  >> cheat
+QED
+
+(* a successful exclusive store has an earlier exclusive load *)
+(* TODO encode success *)
+Theorem is_fulfil_xcl_is_read_xcl:
+  !i tr cid p st t. wf_trace tr /\ SUC i < LENGTH tr
+  /\ is_fulfil_xcl cid t (EL i tr) (FST $ EL (SUC i) tr)
+  /\ FLOOKUP (FST $ EL i tr) cid = SOME $ Core cid p st
+  ==> ?j t. j < i
+    /\ is_read_xcl cid t (EL j tr) (FST $ EL (SUC j) tr)
+    /\ !k p' st'. j < k /\ k <= i
+      /\ FLOOKUP (FST $ EL k tr) cid = SOME $ Core cid p st'
+      ==> st.bst_xclb = st'.bst_xclb
+Proof
+  rpt strip_tac
+  >> drule_then assume_tac is_fulfil_xcl_is_fulfil
+  >> drule_all_then strip_assume_tac is_fulfil_is_promise
+  (* TODO there is a (last) process that sets the exclusive bank *)
+  >> qabbrev_tac `P = λj. 1 < j /\ LENGTH tr - j < i /\ j <= LENGTH tr
+    /\ !st st'. FLOOKUP (FST $ EL (LENGTH tr - j) tr) cid = SOME $ Core cid p st
+      /\ FLOOKUP (FST $ EL (SUC $ LENGTH tr - j) tr) cid = SOME $ Core cid p st'
+      ==> IS_NONE st.bst_xclb /\ IS_SOME st'.bst_xclb`
+  >> Cases_on `?i. P i`
+  >- (
+    dxrule_then assume_tac arithmeticTheory.WOP
+    >> fs[Abbr`P`,DISJ_EQ_IMP,AND_IMP_INTRO]
+    >> drule_then (drule_then $ qspec_then `LENGTH tr - n` assume_tac) wf_trace_cid
+    >> gs[]
+    >> cheat
+    >> `is_read_xcl cid t (EL (LENGTH tr - n) tr) (FST (EL (SUC $ LENGTH tr - n) tr))` by (
+      irule xclb_NONE_SOME_is_read_xclb
+      >> fs[]
+    )
+    >> goal_assum $ drule_at Any
+    (* TODO by xclb_NONE_SOME_is_read_xclb, this is an exclusive load *)
+    >> cheat
+  )
+  >> cheat
+QED
+
+(* fence transitions and their properties *)
+
+Definition is_fence_def:
+  is_fence cid K1 K2 sys1 sys2 <=>
+  ?st st' p.
+    FLOOKUP sys1 cid = SOME $ Core cid p st
+    /\ FLOOKUP sys2 cid = SOME $ Core cid p st'
+    /\ bir_get_stmt p st.bst_pc = BirStmt_Fence K1 K2
+    /\ st'.bst_pc = bir_pc_next st.bst_pc
+    /\ st'.bst_prom = st.bst_prom
+End
+
+Theorem is_fence_parstep_nice:
+  !tr i cid K1 K2.
+    wf_trace tr /\ SUC i < LENGTH tr
+    /\ is_fence cid K1 K2 (FST $ EL i tr) (FST $ EL (SUC i) tr)
+    ==> parstep_nice cid (EL i tr) (EL (SUC i) tr)
+Proof
+  rpt strip_tac
+  >> spose_not_then assume_tac
+  >> drule_all_then strip_assume_tac wf_trace_parstep_EL
+  >> Cases_on `cid = cid'`
+  >> fs[]
+  >> drule wf_trace_NOT_parstep_nice_state_EQ'
+  >> rpt $ disch_then $ drule
+  >> gs[is_fence_def,bir_programTheory.bir_state_t_accfupds,bir_programTheory.bir_pc_next_def,bir_programTheory.bir_programcounter_t_component_equality,parstep_nice_def,parstep_cases,FLOOKUP_UPDATE]
+QED
+
+Theorem is_fence_RW_W_post:
+  !tr i j cid p st st'.
+  wf_trace tr /\ SUC i < LENGTH tr
+  /\ is_fence cid BM_ReadWrite BM_Write (FST $ EL i tr) (FST $ EL (SUC i) tr)
+  /\ FLOOKUP (FST $ EL i tr) cid = SOME $ Core cid p st
+  /\ FLOOKUP (FST $ EL (SUC i) tr) cid = SOME $ Core cid p st'
+  ==>
+    st'.bst_v_rNew = st.bst_v_rNew
+    /\ st'.bst_v_wNew = MAX st.bst_v_wNew $ MAX st.bst_v_rOld st.bst_v_wOld
+Proof
+  rpt gen_tac >> strip_tac
+  >> drule_at_then (Pat `is_fence _ _ _ _ _`) assume_tac is_fence_parstep_nice
+  >> gvs[is_fence_def,parstep_nice_def,parstep_cases,cstep_cases,bir_programTheory.bir_state_t_accfupds,FLOOKUP_UPDATE,clstep_cases,is_read_def,is_write_def]
+QED
+
+(* exclusive bank semantics *)
+
+(*
+ * two distinct cores cid, cid' cannot exclusively fulfil to the same address
+ * if the lr/sc are interleaved.
+ * Here the sc (exclusive fulfil) of cid sees the lr (exclusive read) of cid'
+ *   lr_cid < lr_cid' < sc_cid
+ *)
+Theorem is_fulfil_xcl_is_read_xcl_is_fulfil_xcl:
+  !i j tr cid cid' p st p' st' t t'. wf_trace tr
+  /\ progressing_trace tr
+  /\ is_fulfil_xcl cid t (EL i tr) (FST $ EL (SUC i) tr)
+  /\ FLOOKUP (FST $ EL i tr) cid = SOME $ Core cid p st
+  /\ (THE st.bst_xclb).xclb_time < t
+  /\ (THE st.bst_xclb).xclb_time < LENGTH $ SND $ EL (SUC i) tr
+  /\ PRE t < LENGTH $ SND $ EL (SUC i) tr
+  /\ PRE (THE st.bst_xclb).xclb_time < LENGTH $ SND $ EL (SUC i) tr
+  /\ (0 < (THE st.bst_xclb).xclb_time ==>
+    (EL (PRE (THE st.bst_xclb).xclb_time) (SND (EL (SUC i) tr))).loc
+      = (EL (PRE t) (SND (EL (SUC i) tr))).loc
+    /\ (EL (PRE $ (THE st.bst_xclb).xclb_time) (SND (EL (SUC i) tr))).cid = cid)
+  /\ (EL (PRE t) (SND (EL (SUC i) tr))).cid = cid
+  /\ is_fulfil_xcl cid' t' (EL j tr) (FST $ EL (SUC j) tr)
+  /\ SUC j < LENGTH tr
+  /\ FLOOKUP (FST $ EL j tr) cid' = SOME $ Core cid' p' st'
+  /\ 0 < (THE st'.bst_xclb).xclb_time
+  /\ (THE st'.bst_xclb).xclb_time < t'
+  /\ (THE st'.bst_xclb).xclb_time < LENGTH $ SND $ EL (SUC j) tr
+  /\ PRE t' < LENGTH $ SND $ EL (SUC j) tr
+  /\ (EL (PRE t') (SND (EL (SUC j) tr))).cid = cid'
+  /\ (EL (PRE $ (THE st'.bst_xclb).xclb_time) (SND (EL (SUC j) tr))).cid = cid'
+  /\ (EL (PRE (THE st'.bst_xclb).xclb_time) (SND (EL (SUC j) tr))).loc
+    = (EL (PRE t') (SND (EL (SUC j) tr))).loc
+  /\ cid <> cid'
+  /\ (0 < (THE st.bst_xclb).xclb_time ==>
+    (EL (PRE (THE st.bst_xclb).xclb_time) $ SND $ EL (SUC i) tr).loc
+      = (EL (PRE (THE st'.bst_xclb).xclb_time) $ SND $ EL (SUC j) tr).loc)
+  /\ (EL (PRE t') $ SND $ EL (SUC j) tr).loc
+    = (EL (PRE t) $ SND $ EL (SUC j) tr).loc
+  /\ (THE st.bst_xclb).xclb_time < (THE st'.bst_xclb).xclb_time
+  /\ (THE st'.bst_xclb).xclb_time < t
+  /\ i < j
+  ==> F
+Proof
+  rpt strip_tac
+  >> drule_then (qspecl_then [`SUC j`,`SUC i`] assume_tac) wf_trace_EL_SND_EQ_EL_SND
+  >> drule_at_then (Pos $ el 4) assume_tac is_fulfil_xcl_atomic
+  >> rev_drule_at_then (Pos $ el 4) assume_tac is_fulfil_xcl_atomic
+  >> qmatch_assum_rename_tac `ii < jj:num`
+  >> `SUC ii < SUC jj` by fs[]
+  >> drule_all_then assume_tac wf_trace_IS_PREFIX_SND_EL
+  >> gs[optionTheory.IS_SOME_EXISTS,is_fulfil_xcl_def,IS_PREFIX_APPEND]
+  >> dxrule $ iffLR fulfil_atomic_ok_def
+  >> fs[Once DISJ_COMM,DISJ_EQ_IMP]
+  >> qpat_x_assum `_ < _.xclb_time` $ irule_at Any
+  >> gvs[GSYM arithmeticTheory.PRE_SUB1]
+  >> fs[]
+QED
+
+(*
+ * a successful fulfil t2 with its preceeding read t1
+ *)
+Definition lr_sc_def:
+  lr_sc cid tr t1 i1 t2 i2 <=>
+  SUC i2 < LENGTH tr
+  /\ PRE t2 < LENGTH $ SND $ EL i2 tr
+  /\ is_read_xcl cid t1 (EL i1 tr) (FST $ EL (SUC i1) tr)
+  /\ is_fulfil_xcl cid t2 (EL i2 tr) (FST $ EL (SUC i2) tr)
+  /\ i1 < i2
+  /\ t1 < t2 (* view timestamps strictly ordered *)
+  /\ (* exclusive bank unchanged *)
+    same_state_prop_range cid tr (SUC i1) i2 (λst. st.bst_xclb)
+  /\ (0 < t1 ==>
+    (EL (PRE t1) $ SND $ EL (SUC i1) tr).loc
+    = (EL (PRE t2) $ SND $ EL (SUC i2) tr).loc)
+End
+
+Theorem lr_sc_cid:
+  !tr cid t1 i1 t2 i2.
+  wf_trace tr /\ progressing_trace tr
+  /\ lr_sc cid tr t1 i1 t2 i2
+  ==>
+    (EL (PRE t2) $ SND $ EL (SUC i2) tr).cid = cid
+    /\ (0 < t1
+      ==> (EL (PRE t1) $ SND $ EL i1 tr).cid = cid)
+Proof
+  rpt gen_tac >> strip_tac
+  >> fs[lr_sc_def]
+  >> imp_res_tac is_fulfil_xcl_is_fulfil
+  >> dxrule_at_then (Pat `is_fulfil _ _ _ _`) assume_tac is_fulfil_memory
+  >> gs[is_fulfil_xcl_def,is_read_xcl_def]
+QED
+
+Theorem lr_sc_bst_xclb_eq:
+  !tr cid t1 i1 t2 i2.
+  wf_trace tr
+  /\ lr_sc cid tr t1 i1 t2 i2
+  ==> same_state_prop cid (FST (EL (SUC i1) tr)) (FST (EL i2 tr)) (λst. st.bst_xclb)
+Proof
+  rw[lr_sc_def]
+  >> irule same_state_prop_indexes
+  >> fs[]
+QED
+
+Theorem lr_sc_memory:
+  !tr cid t1 i1 t2 i2.
+  wf_trace tr /\ progressing_trace tr /\ lr_sc cid tr t1 i1 t2 i2
+  ==>
+    SND $ EL i1 tr = SND $ EL (SUC i1) tr
+    /\ SND $ EL i2 tr = SND $ EL (SUC i2) tr
+Proof
+  rpt gen_tac >> strip_tac
+  >> fs[lr_sc_def]
+  >> imp_res_tac is_fulfil_xcl_is_fulfil
+  >> drule_all is_fulfil_memory
+  >> drule_at (Pat `is_read_xcl _ _ _ _`) is_read_xcl_LENGTH_SND_EL
+  >> fs[]
+QED
+
+Theorem lr_sc_same:
+  !tr cid t1 i1 t2 cid' t1' j1 t2' index.
+  wf_trace tr /\ progressing_trace tr
+  /\ lr_sc cid tr t1 i1 t2 index
+  /\ lr_sc cid' tr t1' j1 t2' index
+  ==> cid = cid' /\ t2 = t2'
+Proof
+  rpt gen_tac >> strip_tac
+  >> fs[lr_sc_def]
+  >> imp_res_tac is_fulfil_xcl_is_fulfil
+  >> dxrule_all is_fulfil_same
+  >> fs[]
+QED
+
+Theorem lr_sc_once:
+  !tr cid t1 i1 t2 i2 cid' t1' j1 t2' j2.
+  wf_trace tr /\ progressing_trace tr
+  /\ lr_sc cid tr t1 i1 t2 i2
+  /\ lr_sc cid' tr t1' j1 t2' j2
+  /\ i2 <> j2
+  ==> t2 <> t2'
+Proof
+  rpt strip_tac
+  >> gvs[lr_sc_def]
+  >> imp_res_tac is_fulfil_xcl_is_fulfil
+  >> dxrule_at (Pat `is_fulfil _ _ _ _`) is_fulfil_once
+  >> fs[AC CONJ_ASSOC CONJ_COMM]
+  >> qpat_x_assum `is_fulfil _ _ _ _` $ irule_at Any
+  >> fs[]
+QED
+
+(*
+ * two distinct cores cid, cid' cannot exclusively fulfil to the same address
+ * if the lr/sc are interleaved (t1 < t1' < t2).
+ * The exclusive fulfil to t2 of cid sees the exclusive read of cid' to t1'
+ *)
+Theorem lr_sc_interleaved_pair_i2j2:
+  !tr cid cid' t1 t2 i1 i2 t1' t2' j1 j2.
+  wf_trace tr /\ progressing_trace tr
+  /\ lr_sc cid tr t1 i1 t2 i2
+  /\ lr_sc cid' tr t1' j1 t2' j2
+  /\ t1 < t1' /\ t1' < t2
+  /\ cid <> cid'
+  /\ i2 < j2
+  /\ (EL (PRE t2) $ SND $ EL (SUC i2) tr).loc
+    = (EL (PRE t2') $ SND $ EL (SUC j2) tr).loc
+  ==> F
+Proof
+  rpt strip_tac
+  >> drule_at (Pat `lr_sc _ _ _ _ _ _`) lr_sc_bst_xclb_eq
+  >> rev_drule_at (Pat `lr_sc _ _ _ _ _ _`) lr_sc_bst_xclb_eq
+  >> drule_at (Pat `lr_sc _ _ _ _ _ _`) lr_sc_cid
+  >> rev_drule_at (Pat `lr_sc _ _ _ _ _ _`) lr_sc_cid
+  >> drule_at (Pat `lr_sc _ _ _ _ _ _`) lr_sc_memory
+  >> rev_drule_at (Pat `lr_sc _ _ _ _ _ _`) lr_sc_memory
+  >> rpt strip_tac
+  >> gs[]
+  >> drule_then irule is_fulfil_xcl_is_read_xcl_is_fulfil_xcl
+  >> rev_drule_then (irule_at Any) $ cj 4 $ iffLR lr_sc_def
+  >> drule_then (irule_at Any) $ cj 4 $ iffLR lr_sc_def
+  >> qspecl_then [`tr`,`SUC j1`,`SUC j2`] assume_tac wf_trace_IS_PREFIX_SND_EL'
+  >> qspecl_then [`tr`,`j1`,`SUC j2`] assume_tac wf_trace_IS_PREFIX_SND_EL'
+  >> qspecl_then [`tr`,`SUC i1`,`SUC i2`] assume_tac wf_trace_IS_PREFIX_SND_EL'
+  >> qspecl_then [`tr`,`i1`,`SUC i2`] assume_tac wf_trace_IS_PREFIX_SND_EL'
+  >> qspecl_then [`tr`,`i2`,`j2`] assume_tac wf_trace_IS_PREFIX_SND_EL'
+  >> qspecl_then [`tr`,`j1`,`SUC j1`] assume_tac wf_trace_memory_LENGTH
+  >> qspecl_then [`tr`,`i1`,`SUC i1`] assume_tac wf_trace_memory_LENGTH
+  >> qspecl_then [`i1`,`i2`,`tr`,`cid`] assume_tac wf_trace_cid_backward
+  >> qspecl_then [`j1`,`j2`,`tr`,`cid'`] assume_tac wf_trace_cid_backward
+  >> gs[lr_sc_def]
+  >> Cases_on `0 < t1`
+  >> gvs[same_state_prop_def,is_fulfil_xcl_def,is_read_xcl_def,IS_PREFIX_EL]
+  >> conj_asm1_tac
+  >- gs[IS_PREFIX_LENGTH,arithmeticTheory.PRE_SUB1]
+  >> rpt $ dxrule_then assume_tac IS_PREFIX_EL
+  >> gs[]
+QED
+
+(*
+ * two distinct cores cid, cid' cannot exclusively fulfil to the same address
+ * if the lr/sc are interleaved (t1 < t1' < t2)
+ * The exclusive fulfil to t2 of cid sees the exclusive write of cid to t2'
+ *)
+Theorem lr_sc_interleaved_pair_j2i2:
+  wf_trace tr
+  /\ progressing_trace tr
+  /\ lr_sc cid tr t1 i1 t2 i2
+  /\ lr_sc cid' tr t1' j1 t2' j2
+  /\ t1 < t1'
+  /\ t1' < t2
+  /\ cid <> cid'
+  /\ (EL (PRE t2) (SND (EL (SUC i2) tr))).loc = (EL (PRE t2') (SND (EL (SUC j2) tr))).loc
+  /\ j2 < i2
+  ==> F
+Proof
+  rpt strip_tac
+  >> `?p st. FLOOKUP (FST (EL i2 tr)) cid = SOME (Core cid p st)
+        /\ fulfil_atomic_ok (SND (EL (SUC i2) tr))
+          (EL (PRE t2) (SND (EL (SUC i2) tr))).loc cid st t2
+        /\ IS_SOME st.bst_xclb
+    ` by (
+    fs[lr_sc_def]
+    >> rev_drule_at_then (Pat `is_fulfil_xcl _ _ _ _`) assume_tac $ cj 1 is_fulfil_xcl_atomic
+    >> gs[is_fulfil_xcl_def]
+  )
+  >> qhdtm_x_assum `fulfil_atomic_ok` mp_tac
+  >> fs[fulfil_atomic_ok_def,optionTheory.IS_SOME_EXISTS,Once DISJ_COMM,DISJ_EQ_IMP,NOT_ZERO_LT_ZERO]
+  >> `x.xclb_time = t1` by (
+    rev_drule_at_then (Pat `lr_sc _ _ _ _ _ _`) assume_tac lr_sc_bst_xclb_eq
+    >> rev_dxrule_then strip_assume_tac $ iffLR lr_sc_def
+    >> qspecl_then [`i1`,`i2`,`tr`,`cid`] assume_tac wf_trace_cid_backward
+    >> gvs[is_read_xcl_def,same_state_prop_def]
+  )
+  >> conj_asm1_tac
+  >- (
+    strip_tac
+    >> rev_dxrule_then strip_assume_tac $ iffLR lr_sc_def
+    >> qspecl_then [`tr`,`SUC i1`,`SUC i2`] assume_tac wf_trace_IS_PREFIX_SND_EL
+    >> drule_at_then (Pat `is_read_xcl _ _ _ _`) assume_tac is_read_xcl_LENGTH_SND_EL
+    >> `PRE t1 < LENGTH $ SND $ EL (SUC i1) tr /\ j1 < j2` by (
+      gs[lr_sc_def,is_read_xcl_def]
+    )
+    >> gs[GSYM PRE_SUB1,EL_APPEND1,is_read_xcl_def,IS_PREFIX_APPEND]
+  )
+  >> fs[AC CONJ_ASSOC CONJ_COMM]
+  >> goal_assum rev_drule
+  >> fs[GSYM PRE_SUB1]
+  >> `SUC i2 < LENGTH tr` by fs[lr_sc_def,is_fulfil_xcl_def]
+  >> conj_tac
+  >- (
+    fs[]
+    >> dxrule_then strip_assume_tac $ iffLR lr_sc_def
+    >> qpat_x_assum `_:num <> _` mp_tac
+    >> qspecl_then [`tr`,`j1`,`SUC i2`] assume_tac wf_trace_IS_PREFIX_SND_EL
+    >> gvs[is_read_xcl_def,IS_PREFIX_APPEND,EL_APPEND1]
+  )
+  >> dxrule_then strip_assume_tac $ iffLR lr_sc_def
+  >> qspecl_then [`tr`,`SUC j1`,`SUC j2`] assume_tac wf_trace_IS_PREFIX_SND_EL
+  >> qspecl_then [`tr`,`SUC j2`,`SUC i2`] assume_tac wf_trace_IS_PREFIX_SND_EL
+  >> drule_at_then (Pat `is_read_xcl _ _ _ _`) assume_tac is_read_xcl_LENGTH_SND_EL
+  >> gs[EL_APPEND1,IS_PREFIX_APPEND,is_read_xcl_def]
+QED
+
+(* disallowed interleaving if t1 < t1' < t2 *)
+
+Theorem lr_sc_interleaved_pair:
+  !tr cid cid' t1 t2 i1 i2 t1' t2' j1 j2.
+  wf_trace tr /\ progressing_trace tr
+  /\ lr_sc cid tr t1 i1 t2 i2
+  /\ lr_sc cid' tr t1' j1 t2' j2
+  /\ t1 < t1' /\ t1' < t2
+  /\ cid <> cid'
+  /\ (EL (PRE t2) $ SND $ EL (SUC i2) tr).loc
+    = (EL (PRE t2') $ SND $ EL (SUC j2) tr).loc
+  ==> F
+Proof
+  rpt strip_tac
+  >> Cases_on `i2 < j2`
+  >- (drule_all_then irule lr_sc_interleaved_pair_i2j2)
+  >> reverse $ fs[NOT_LESS,LESS_OR_EQ]
+  >- (gvs[] >> dxrule_all lr_sc_same >> fs[])
+  >> drule_all lr_sc_interleaved_pair_j2i2
+  >> fs[]
+QED
+
+(* disallowed interleaving if t1 < t2' < t2 *)
+
+Theorem lr_sc_interleaved_pair':
+  !tr cid cid' t1 t2 i1 i2 t1' t2' j1 j2.
+  wf_trace tr /\ progressing_trace tr
+  /\ lr_sc cid tr t1 i1 t2 i2
+  /\ lr_sc cid' tr t1' j1 t2' j2
+  /\ t1 < t2'
+  /\ t2' < t2
+  /\ cid <> cid'
+  /\ (EL (PRE t2) $ SND $ EL (SUC i2) tr).loc
+    = (EL (PRE t2') $ SND $ EL (SUC j2) tr).loc
+  ==> F
+Proof
+  rpt strip_tac
+  >> `?p st. FLOOKUP (FST (EL i2 tr)) cid = SOME (Core cid p st)
+        /\ fulfil_atomic_ok (SND (EL (SUC i2) tr))
+          (EL (PRE t2) (SND (EL (SUC i2) tr))).loc cid st t2
+        /\ IS_SOME st.bst_xclb
+    ` by (
+    fs[lr_sc_def]
+    >> rev_drule_at_then (Pat `is_fulfil_xcl _ _ _ _`) assume_tac $ cj 1 is_fulfil_xcl_atomic
+    >> gs[is_fulfil_xcl_def]
+  )
+  >> qhdtm_x_assum `fulfil_atomic_ok` mp_tac
+  >> fs[fulfil_atomic_ok_def,optionTheory.IS_SOME_EXISTS,Once DISJ_COMM,DISJ_EQ_IMP,NOT_ZERO_LT_ZERO]
+  >> `x.xclb_time = t1` by (
+    rev_drule_at_then (Pat `lr_sc _ _ _ _ _ _`) assume_tac lr_sc_bst_xclb_eq
+    >> rev_dxrule_then strip_assume_tac $ iffLR lr_sc_def
+    >> qspecl_then [`i1`,`i2`,`tr`,`cid`] assume_tac wf_trace_cid_backward
+    >> gvs[is_read_xcl_def,same_state_prop_def]
+  )
+  >> conj_asm1_tac
+  >- (
+    strip_tac
+    >> rev_dxrule_then strip_assume_tac $ iffLR lr_sc_def
+    >> qspecl_then [`tr`,`SUC i1`,`SUC i2`] assume_tac wf_trace_IS_PREFIX_SND_EL
+    >> drule_at_then (Pat `is_read_xcl _ _ _ _`) assume_tac is_read_xcl_LENGTH_SND_EL
+    >> `PRE t1 < LENGTH $ SND $ EL (SUC i1) tr /\ i1 < i2` by (
+      gs[lr_sc_def,is_read_xcl_def]
+    )
+    >> gs[GSYM PRE_SUB1,EL_APPEND1,is_read_xcl_def,IS_PREFIX_APPEND]
+  )
+  >> fs[AC CONJ_ASSOC CONJ_COMM]
+  >> goal_assum rev_drule
+  >> fs[GSYM PRE_SUB1]
+  >> `SUC i2 < LENGTH tr /\ SUC j2 < LENGTH tr` by fs[lr_sc_def,is_fulfil_xcl_def]
+  >> imp_res_tac $ cj 4 $ iffLR lr_sc_def
+  >> ntac 2 $ dxrule_then assume_tac is_fulfil_xcl_is_fulfil
+  >> ntac 2 $ dxrule_at_then (Pat `is_fulfil`) assume_tac is_fulfil_to_memory
+  >> qpat_x_assum `_:num <> _` mp_tac
+  >> gvs[]
+  >> cheat (* both PRE t2 and PRE t2' are smaller than the memory SND $ EL (MIN i2 j2) *)
+QED
+
+val _ = export_theory();
